{"nbformat":4,"nbformat_minor":0,"metadata":{"colab":{"provenance":[],"authorship_tag":"ABX9TyMdCZ1Dip9VuvZdM8x1JNxT"},"kernelspec":{"name":"python3","display_name":"Python 3"},"language_info":{"name":"python"}},"cells":[{"cell_type":"markdown","source":["#Introduction of Exponential function"],"metadata":{"id":"QR3q4wYTsETz"}},{"cell_type":"markdown","source":["###(0) Triangle of Power (3Blue1Brown)\n","\n","* reference: https://youtu.be/sULa9Lc4pck"],"metadata":{"id":"J8_RZXUY3yRq"}},{"cell_type":"markdown","source":["**Notation**\n","* $\\frac{[a]}{[b][]}=b^a$\n","* $\\frac{[]}{[b][c]}=\\log_{b}c$\n","* $\\frac{[a]}{[][c]}=(c)^{\\frac{1}{a}}$\n","\n","**Operation**\n","* $\\frac{[+]}{[\\mathbb{R}][\\times]}$\n","* $\\frac{[y_1]}{[x][]}*\\frac{[y_2]}{[x][]}=x^{y_1}*x^{y_2}=x^{y_1+y_2}$\n","* $\\frac{[]}{[x][y_1]}+\\frac{[]}{[x][y_1]}=\\log_{x}y_1+\\log_{x}y_2=\\log_{x}(y_1*y_2)$\n","\n","**Identity**\n","* $\\frac{[\\frac{[]}{[b][c]}]}{[b][]}=b^{\\log_{b}c}=c$\n","* etc."],"metadata":{"id":"viUyCB436_fx"}},{"cell_type":"markdown","source":["###(1) $a^b=c \\implies \\log_ac=b$"],"metadata":{"id":"U1AQsJV-ehGw"}},{"cell_type":"markdown","source":["Types of $\\log_ab$\n","1. Logarithm = $\\log_ab$\n","2. Common Logarithm = $\\log_{10}b=\\log b$\n","3. Natural Logarithm = $\\log_eb=\\ln b$"],"metadata":{"id":"gulV-qn9g9ta"}},{"cell_type":"markdown","source":["Properties\n","* $\\log_ab > 0$\n","* $\\log_aa^x=x$\n","* $a^{\\log_ax}=x$\n","* $\\log_a1=0$"],"metadata":{"id":"N0osngf_wq4H"}},{"cell_type":"markdown","source":["Property of $f(x)=\\log_a(mx+c)$\n","\n","1. Domain (the domain of a function is the set of inputs accepted by the function.)\n","\n","* $mx+c>0$\n","\n","$mx>-c$\n","\n","* If $m>0 \\implies x>\\frac{-c}{|m|} \\therefore$ Domain = $(\\frac{-c}{|m|},\\infty)$\n","\n","* If $m<0 \\implies x<\\frac{-c}{-|m|} \\implies x<\\frac{c}{|m|}$ Domain = $(-\\infty, \\frac{c}{|m|})$\n","\n","2. Range = the difference between the largest and smallest value of $f(x)$. \n","\n","* In this case, range = $(-\\infty,\\infty)$\n","\n","3. Asymptote = a line or curve that acts as the limit of another line or curve. \n","\n","* Horizontal Asymptote = $\\infty$\\\n","\n","* If $m>0 \\implies$ Vertical Asymptote = $\\frac{-c}{|m|}$\n","\n","* If $m<0 \\implies$ Vertical Asymptote = $\\frac{c}{|m|}$"],"metadata":{"id":"kqWZH0tAkugz"}},{"cell_type":"markdown","source":["Example:\n","* $\\log_216=4$\n","* $\\log_381=4$\n","* $\\log_{10}-100=$ Undefined.\n","* $\\log_70=$ Undefined.\n","* etc."],"metadata":{"id":"vvurHEExf1t0"}},{"cell_type":"markdown","source":["###(2) Rules of $\\log$"],"metadata":{"id":"_geusCTKw0pT"}},{"cell_type":"markdown","source":["**Exponential Rules**\n","* $a^0=1$\n","* $a^m*a^n=a^{m+n}$\n","* $\\frac{a^m}{a^n}=a^m*a^{-n}=a^{m-n}$\n","* $(a^m)^n=a^{m*n}$"],"metadata":{"id":"2kshkzsrw6YX"}},{"cell_type":"markdown","source":["**Logarithm Rules**\n","* $\\log_a(1)=0$\n","* $\\log_a(xy)=\\log_a(x)+\\log_a(y)$\n","* $\\log_a(\\frac{x}{y})=\\log_a(x)-\\log_a(y)$\n","* $\\log_a(x^y)=y*\\log_a(x)=\\log_a(x)*y$\n","* $\\log_ab=\\frac{1}{\\log_ba}$"],"metadata":{"id":"xULg-PqfyCEA"}},{"cell_type":"markdown","source":["**Prove that $\\log_a(xy)=\\log_a(x)+\\log_a(y)$:**\n","\n","Let \n","* $x_u=\\log_a(x) \\therefore a^{x_u}=x$\n","* $y_u=\\log_a(y) \\therefore a^{y_u}=y$\n","* $b=\\log_a(\\frac{x}{y})$\n","\n","$a^{b}=xy=a^{x_u}*a^{y_u}=a^{x_u+y_u}$\n","\n","$\\therefore b=x_u+y_u=\\log_a(xy)=\\log_a(x)+\\log_a(y)$\n","\n","reference: https://math.stackexchange.com/questions/2002721/proof-of-logxy-log-x-log-y"],"metadata":{"id":"c9yNa8Xz5qRJ"}},{"cell_type":"markdown","source":["**Prove that $\\log_a(\\frac{x}{y})=\\log_a(x)-\\log_a(y)$:**\n","\n","Let \n","* $x_u=\\log_a(x) \\therefore a^{x_u}=x$\n","* $y_u=\\log_a(y) \\therefore a^{y_u}=y$\n","* $b=\\log_a(\\frac{x}{y})$\n","\n","$a^b=\\frac{x}{y}=\\frac{a^{x_u}}{a^{y_u}}=a^{x_u-y_u}$\n","\n","$\\therefore b = x_u-y_u = \\log_a(\\frac{x}{y})=\\log_a(x)-\\log_a(y)$"],"metadata":{"id":"gHkotCUX-ykX"}},{"cell_type":"markdown","source":["**Prove that $\\log_a(x^y)=y*\\log_a(x)=\\log_a(x)*y$:**\n","\n","Let \n","* $x_u=\\log_a(x) \\therefore a^{x_u}=x$\n","\n","$(a^{x_u})^n=a^{x_u*n}=x^n$\n","\n","$\\therefore \\log_a(x^n)=x_u*n=\\log_a(x)*n$"],"metadata":{"id":"pqI7uNtB_8KP"}},{"cell_type":"markdown","source":["**Prove that: $\\log_ab=\\frac{1}{\\log_ba}$**\n","\n","Given that:\n","* $a^b=c\\implies\\log_ac=b$\n","\n","$a=c^\\frac{1}{b}$\n","\n","$\\therefore\\log_ca=\\frac{1}{b}=\\frac{1}{\\log_ac}$"],"metadata":{"id":"nDy8CuJ6qaQX"}},{"cell_type":"markdown","source":["###What is $e\\,?$ , $e=\\lim_{n\\to\\infty}(1+\\frac{1}{n})^n$"],"metadata":{"id":"r6G0BZOq2tn6"}},{"cell_type":"markdown","source":["Property $e$\n","\n","1. $\\lim_{n \\to \\infty}(1+\\frac{1}{n})^n=e$\n","2. $\\lim_{h \\to 0}\\frac{e^{h}-1}{h}=1$\n","3. $\\frac{d}{dx}[e^x] = \\lim_{h \\to 0}\\frac{e^{x+h}-e^x}{h} = e^x\\lim_{h \\to 0}\\frac{e^{h}-1}{h} = e^x$"],"metadata":{"id":"5F35d7Gqw28x"}}]}