{"nbformat":4,"nbformat_minor":0,"metadata":{"colab":{"provenance":[],"authorship_tag":"ABX9TyM10t3J0Hlypz4F8L75LYiC"},"kernelspec":{"name":"python3","display_name":"Python 3"},"language_info":{"name":"python"}},"cells":[{"cell_type":"markdown","source":["###(1) implicit differentiation"],"metadata":{"id":"bDj4rBpdV0sl"}},{"cell_type":"markdown","source":["**Note:**\n","\n","In order to find $\\frac{d}{dx}[f(x)]$, \n","1. view other variable that is related to $x$, a.k.a. $y$ as inner function a.k.a. $y= g(x)$\n","2. $\\frac{d}{dx}[y]=\\frac{d}{dx}[g(x)]=\\frac{dy}{dx}$"],"metadata":{"id":"9HREQYZGlkXm"}},{"cell_type":"markdown","source":["**Example No.1**\n","\n","Finding $\\frac{dy}{dx}$ of $x^2+y^2=1$\n","\n","$\\frac{dy}{dx}[x^2+y^2]=\\frac{dy}{dx}[1]$\n","\n","$\\frac{dy}{dx}[x^2+y^2]=0$\n","\n","According to Sum Rule: $\\frac{d}{dx}[f(x)+g(x)] = \\frac{d}{dx}f(x)+\\frac{d}{dx}g(x)$\n","\n","$\\frac{dy}{dx}[x^2]+\\frac{dy}{dx}[y^2]=0$\n","\n","$2x+\\frac{dy}{dx}[y^2]=0$\n","\n","Given that:\n","* $y\\text{ is a function that take $x$ as its input}\\implies y=g(x)\\implies y^2\\text{ is a nested function}\\implies y^2=f(g(x))$\n","* $f(x)=x^2$\n","* $g(x)=y$\n","* $\\frac{d}{dx}[g(x)]=\\frac{dy}{dx}$\n","* $\\therefore f(g(x))=g(x)^2$\n","\n","According to Chain Rule: $\\frac{d}{dx}[f(g(x))] = (f\\circ g)'= f'(g(x))*g'(x)$\n","* $\\therefore \\frac{d}{dx}[y^2]=\\frac{d}{dx}[f(g(x))]= f'(g(x))*g'(x)=2g(x)*g'(x)=2y*\\frac{dy}{dx}$\n","\n","$\\therefore 2x+2y*\\frac{dy}{dx}=0$\n","\n","$x+y*\\frac{dy}{dx}=0$\n","\n","$y*\\frac{dy}{dx}=-x$\n","\n","$\\therefore\\frac{dy}{dx}=\\frac{-x}{y}$"],"metadata":{"id":"y_v5Ty7fWsss"}},{"cell_type":"markdown","source":["**Example No.2**\n","\n","Finding $\\frac{d}{dx}$ of $x^2y-y^2x^3=3$\n","\n","$\\frac{d}{dx}[x^2y-y^2x^3]=\\frac{d}{dx}[3]$\n","\n","$\\frac{d}{dx}[x^2y]-\\frac{d}{dx}[y^2x^3]=0$\n","\n","Given that\n","* $y=g(x)$\n","* $\\frac{d}{dx}[y]=\\frac{dy}{dx}=\\frac{d}{dx}[g(x)]$\n","\n","$\\therefore \\frac{d}{dx}[x^2g(x)]+\\frac{d}{dx}[-g(x)^2x^3]=0$\n","\n","According to Product Rule: $\\frac{d}{dx}[f(x)*g(x)] = f'(x)*g(x)+g'(x)*f(x)$\n","\n","$\\therefore \\frac{d}{dx}[x^2]*g(x)+\\frac{d}{dx}[g(x)]*x^2+\\frac{d}{dx}[-g(x)^2]x^3+\\frac{d}{dx}[x^3]*(-g(x)^2)=0$\n","\n","$\\therefore \\frac{d}{dx}[x^2]*g(x)+\\frac{d}{dx}[g(x)]*x^2+\\frac{d}{dx}[-g(x)^2]x^3+\\frac{d}{dx}[x^3]*(-g(x)^2)=0$\n","\n","According to Power Rule: $f'(x^n) = nx^{n-1}$\n","\n","$\\therefore 2x*g(x)+\\frac{d}{dx}[g(x)]*x^2+\\frac{d}{dx}[-g(x)^2]x^3+3x^2*(-g(x)^2)=0$\n","\n","According to Chain Rule: $\\frac{d}{dx}[f(g(x))] = (f\\circ g)'= f'(g(x))*g'(x)$\n","\n","Given that:\n","* $\\frac{d}{dx}[-g(x)^2]=-2g(x)\\frac{d}{dx}[g(x)]$\n","\n","$\\therefore 2x*g(x)+\\frac{d}{dx}[g(x)]*x^2+(-2g(x)\\frac{d}{dx}[g(x)])*x^3+3x^2*(-g(x)^2)=0$\n","\n","$2x*g(x)+\\frac{d}{dx}[g(x)]*x^2-2g(x)\\frac{d}{dx}[g(x)]*x^3-3x^2*g(x)^2=0$\n","\n","$2x*y+\\frac{dy}{dx}*x^2-2y\\frac{dy}{dx}*x^3-3x^2*y^2=0$\n","\n","$\\frac{dy}{dx}*x^2-2y\\frac{dy}{dx}*x^3=3x^2*y^2-2x*y$\n","\n","$x^2\\frac{dy}{dx}-2yx^3\\frac{dy}{dx}=3x^2*y^2-2x*y$\n","\n","$(x^2-2yx^3)\\frac{dy}{dx}=3x^2*y^2-2x*y$\n","\n","$\\therefore \\frac{dy}{dx}=\\frac{3x^2*y^2-2x*y}{x^2-2yx^3}$\n"],"metadata":{"id":"sPwdxy-zXSvx"}},{"cell_type":"markdown","source":["reference:\n","* https://youtu.be/eenHMD4zDAY\n","* https://www.khanacademy.org/math/ap-calculus-ab/ab-differentiation-2-new/ab-3-2/a/implicit-differentiation-review"],"metadata":{"id":"d2O-01mcV2dG"}}]}