{"nbformat":4,"nbformat_minor":0,"metadata":{"colab":{"provenance":[],"collapsed_sections":["YZovfdgh0pAn","xDMH0NmE0Ui2","RNh7jF5Z9Oor","2PqKfFaM5Amr","ago0fZlawozN","9HEMhras8fNe","HLh6U2yywxEV","F1ZRSksg2wBY","tFUskp69UuJe","68lYTFD0T63X","WYrG-2fT5cWx","Vo7n_5EZFt91","5hYfZY41Hc9a"],"authorship_tag":"ABX9TyOQkME+B8n4DPgm5+C7/mYG"},"kernelspec":{"name":"python3","display_name":"Python 3"},"language_info":{"name":"python"}},"cells":[{"cell_type":"markdown","source":["###(0) Constant Rule, $f'(x)=0 $, {$ x = c$}"],"metadata":{"id":"YZovfdgh0pAn"}},{"cell_type":"markdown","source":["$f'(x)=0 $, {$ x = c$}"],"metadata":{"id":"qqmteXVJ2imV"}},{"cell_type":"markdown","source":["Prove:\n","\n","$f(x)=10$\n","\n","$f'(x) = \\lim_{h\\to 0} \\frac{10-10}{h} = 0$"],"metadata":{"id":"0QZrkBLH2jLD"}},{"cell_type":"markdown","source":["###(1) Sum Rule, $\\frac{d}{dx}[f(x)+g(x)] = \\frac{d}{dx}f(x)+\\frac{d}{dx}g(x)$"],"metadata":{"id":"xDMH0NmE0Ui2"}},{"cell_type":"markdown","source":["$\\frac{d}{dx}[f(x)+g(x)] = \\frac{d}{dx}f(x)+\\frac{d}{dx}g(x)$\n","\n","$\\frac{d}{dx}[f(x)-g(x)] = \\frac{d}{dx}f(x)-\\frac{d}{dx}g(x)$\n"],"metadata":{"id":"4C-2uZKS25KA"}},{"cell_type":"markdown","source":["Prove No.1:\n","\n","$f(x)=u(x)+v(x)$\n","\n","$f'(x) = \\lim_{h\\to 0} \\frac{f(x+h)-f(x)}{h}$\n","\n","$= \\lim_{h\\to 0} \\frac{u(x+h)+v(x+h)-u(x)-v(x)}{h}$\n","\n","$= \\lim_{h\\to 0} \\frac{u(x+h)-u(x)+v(x+h)-v(x)}{h}$\n","\n","$= \\lim_{h\\to 0} \\frac{u(x+h)-u(x)}{h}+\\frac{v(x+h)-v(x)}{h}$\n","\n","$= \\lim_{h\\to 0} \\frac{u(x+h)-u(x)}{h}+\\lim_{h\\to 0} \\frac{v(x+h)-v(x)}{h}$\n","\n","$= u'(x) + v'(x)$\n","\n","$\\therefore f'(x)=u'(x)+v'(x)$"],"metadata":{"id":"3XxZiUpY25rN"}},{"cell_type":"markdown","source":["reference:\n","* https://youtu.be/hZAS9ilEbEE\n","* https://www.khanacademy.org/math/old-ap-calculus-ab/ab-derivative-rules/ab-basic-diff-rules/a/basic-differentiation-review"],"metadata":{"id":"cwb2ylXo9FZm"}},{"cell_type":"markdown","source":["###(2) Constant multiple rule No.1, $\\frac{d}{dx}[k*f(x)] = k*\\frac{d}{dx}f(x)$"],"metadata":{"id":"RNh7jF5Z9Oor"}},{"cell_type":"markdown","source":["Prove that $\\frac{d}{dx}[k*f(x)] = k*\\frac{d}{dx}f(x),$ No.1:\n","\n","$f(x)=k*g(x)$\n","\n","$f'(x) = \\lim_{h\\to 0} \\frac{f(x+h)-f(x)}{h}$\n","\n","$= \\lim_{h\\to 0} \\frac{k*g(x+h)-k*g(x)}{h}$\n","\n","$= k*\\lim_{h\\to 0} \\frac{g(x+h)-g(x)}{h}$\n","\n","$\\therefore \\frac{dx}{dy}[k*g(x)]=k*g'(x)$"],"metadata":{"id":"AE0aZZi49yui"}},{"cell_type":"markdown","source":["Prove that $f'(nx+c) = n$:\n","\n","$f(x) = nx+c$\n","\n","$f'(x) = \\lim_{h\\to 0} \\frac{f(x+h)-f(x)}{h}$\n","\n","$= \\lim_{h\\to 0} \\frac{(n(x+h)+c)-(n(x)+c)}{h}$\n","\n","$= \\lim_{h\\to 0} \\frac{nx+nh+c-nx-c}{h}$\n","\n","$= \\lim_{h\\to 0} \\frac{nh}{h}$\n","\n","$= \\lim_{h\\to 0} n$\n","\n","$\\therefore f'(nx) = n$"],"metadata":{"id":"lLFOV8Bh5SDD"}},{"cell_type":"markdown","source":["###(3) Power Rule: $f'(x^n) = nx^{n-1}$"],"metadata":{"id":"ago0fZlawozN"}},{"cell_type":"markdown","source":["Prove that $f'(x^n) = nx^{n-1}$:\n","\n","\n","$f(x) = x^n$\n","\n","$f'(x) = \\lim_{h\\to 0} \\frac{f(x+h)-f(x)}{h}$\n","\n","$= \\lim_{h\\to 0} \\frac{(x+h)^n-(x)^n}{h}$\n","\n","$= \\lim_{h\\to 0} \\frac{(x)^n+nhx^{n-1}+h^2(...)-(x)^n}{h}$\n","\n","$= \\lim_{h\\to 0} \\frac{nhx^{n-1}+h^2(...)}{h}$\n","\n","$= \\lim_{h\\to 0} {nx^{n-1}+h(...)}$\n","\n","$\\therefore f'(x^n) = nx^{n-1}$"],"metadata":{"id":"g_aAgTu20v49"}},{"cell_type":"markdown","source":["Warning No.1:\n","\n","$\\frac{d}{dx}[(ax+b)^c] \\neq c(ax+b)^{c-1}$\n","\n","$\\frac{d}{dx}[(ax+b)^c] = ac(ax+b)^{c-1}$\n","\n","Example No.1:\n","\n","$\\frac{d}{dx}[(3-x)^{\\frac{-1}{2}}] = \\frac{-1}{2}*-1*(3-x)^{\\frac{-3}{2}} = \\frac{1}{2}*(3-x)^{\\frac{-3}{2}}$"],"metadata":{"id":"6natPCBkhe40"}},{"cell_type":"markdown","source":["Prove that $\\frac{d}{dx}[x^{-n}]=-n*x^{-n-1}:$\n","\n","$f(x)= x^{\\frac{1}{n}}$\n","\n","$f'(x)=\\lim_{h\\to 0}\\frac{(x+h)^{-n}-x^{-n}}{h}$\n","\n","$=\\lim_{h\\to 0}\\frac{\\frac{1}{(x+h)^{n}}-\\frac{1}{x^{n}}}{h}$\n","\n","$=\\lim_{h\\to 0}\\frac{(x)^{n}-(x+h)^{n}}{h*(x+h)^{n}*(x)^{n}}$\n","\n","$=\\lim_{h\\to 0}\\frac{(x)^{n}-x^n-nhx^{n-1}-h^2(...)}{h*(x^n+nhx^{n-1}+h^2(...))*(x)^{n}}$\n","\n","$=\\lim_{h\\to 0}\\frac{-nhx^{n-1}-h^2(...)}{h*(x^n+nhx^{n-1}+h^2(...))*(x)^{n}}$\n","\n","$=\\lim_{h\\to 0}\\frac{-nx^{n-1}-h(...)}{(x^n+nhx^{n-1}+h^2(...))*(x)^{n}}$\n","\n","$=\\lim_{h\\to 0}\\frac{-nx^{n-1}-0}{(x^n+0)*(x)^{n}}$\n","\n","$=\\lim_{h\\to 0}\\frac{-nx^{n-1}}{x^{2n}}$\n","\n","$=\\lim_{h\\to 0}-nx^{n-1-2n}$\n","\n","$=\\lim_{h\\to 0}-nx^{-1-n}$"],"metadata":{"id":"E4ijCyOP54_z"}},{"cell_type":"markdown","source":["Prove that $\\frac{d}{dx}[(ax+b)^c] = ac(ax+b)^{c-1}$:\n","\n","$f(x)=x^c$\n","\n","$g(x)=ax+b$\n","\n","$f(g(x)) = (ax+b)^c$\n","\n","According to Chain Rule: $\\frac{d}{dx}[f(g(x))] = f'(g(x))*g'(x)$\n","\n","$\\frac{d}{dx}[f(g(x))] = c(ax+b)^{c-1}*a*1*x^{1-1}$\n","\n","$\\therefore \\frac{d}{dx}[f(g(x))] = ac(ax+b)^{c-1}$"],"metadata":{"id":"T1EmVcaOG6mY"}},{"cell_type":"markdown","source":["Prove that $f'(ax^n) = anx^{n-1}$:\n","\n","$f(x)=ax^n$\n","\n","$f'(x) = \\lim_{h\\to 0} \\frac{f(x+h)-f(x)}{h}$\n","\n","$= \\lim_{h\\to 0} \\frac{a(x+h)^n-a(x)^n}{h}$\n","\n","$= \\lim_{h\\to 0} \\frac{a(x)^n+anhx^{n-1}+ah^2(...)-a(x)^n}{h}$\n","\n","$= \\lim_{h\\to 0} \\frac{anhx^{n-1}+h^2(...)}{h}$\n","\n","$= \\lim_{h\\to 0} {anx^{n-1}+h(...)}$\n","\n","$\\therefore f'(ax^n) = anx^{n-1}$"],"metadata":{"id":"DeMlQgj98wxr"}},{"cell_type":"markdown","source":["###(4) $\\frac{d}{dx}[e^x] =e^x$"],"metadata":{"id":"HLh6U2yywxEV"}},{"cell_type":"markdown","source":["**Prove that: $\\frac{d}{dx}[e^x]=e^x$**\n","\n","Property $e$\n","\n","1. $\\lim_{n \\to \\infty}(1+\\frac{1}{n})^n=e$\n","2. $\\lim_{h \\to 0}\\frac{e^{h}-1}{h}=1$\n","\n","\n","$\\therefore\\frac{d}{dx}[e^x] = \\lim_{h \\to 0}\\frac{e^{x+h}-e^x}{h} = e^x\\lim_{h \\to 0}\\frac{e^{h}-1}{h} = e^x$"],"metadata":{"id":"5F35d7Gqw28x"}},{"cell_type":"markdown","source":["**Prove that $\\lim_{h \\to 0}\\frac{e^{h}-1}{h}=1$ No.1:**\n","\n","Given that\n","* $y=e^h-1$\n","\n","$\\therefore y+1=e^h$\n","\n","$\\log_e(y+1)=\\log_e(e^h)$\n","\n","According to Logarithm property: $\\log_aa^x=x$\n","\n","$\\therefore \\log_e(y+1)=h$\n","\n","Given that\n","* $y=e^h-1$\n","* $\\log_e(y+1)=h$\n","\n","$\\therefore \\frac{e^{h}-1}{h}=\\frac{y}{\\log_e(y+1)}=\\frac{e^{h}-1}{\\log_e(e^h-1+1)}$\n","\n","Given that:\n","* $\\lim_{h\\to0}e^h-1=\\lim_{y\\to0}y$\n","\n","$\\therefore \\lim_{h\\to0}\\frac{e^{h}-1}{h}=\\lim_{y\\to0}\\frac{y}{\\log_e(y+1)}$\n","\n","$\\lim_{y\\to0}\\frac{y}{\\ln(y+1)}=\\lim_{y\\to0}\\frac{1}{\\frac{\\ln(y+1)}{y}}$\n","\n","$\\lim_{y\\to0}\\frac{y}{\\ln(y+1)}=\\lim_{y\\to0}\\frac{1}{\\frac{1}{y}*\\ln(y+1)}$\n","\n","\n","According to Logarithm property: $\\log_a(x^y)=y*\\log_a(x)=\\log_a(x)*y$\n","\n","$\\therefore\\lim_{y\\to0}\\frac{y}{\\ln(y+1)}=\\lim_{y\\to0}\\frac{1}{\\ln((y+1)^\\frac{1}{y})}$\n","\n","Given that\n","* $\\lim_{n\\to\\infty}(1+\\frac{1}{n})^n=e$\n","* $\\lim_{n\\to\\infty}\\frac{1}{n}=\\lim_{y\\to0}y$\n","* $\\therefore \\lim_{n\\to\\infty}(1+\\frac{1}{n})^n=\\lim_{y\\to0}(y+1)^\\frac{1}{y}=e$\n","\n","$\\therefore\\lim_{y\\to0}\\frac{y}{\\ln(y+1)}=\\frac{1}{\\ln(e)}$\n","\n","According to Logarithm property: $\\log_aa^x=x$\n","\n","$\\therefore\\lim_{y\\to0}\\frac{y}{\\ln(y+1)}=\\frac{1}{1}=1$\n","\n","reference:\n","* https://youtu.be/qWw8VnzTddg\n","* https://socratic.org/questions/how-do-you-solve-the-following-limit-e-x-1-x-as-x-approaches-zero"],"metadata":{"id":"7rJUQgU0Xohu"}},{"cell_type":"markdown","source":["**Prove that $\\lim_{h \\to 0}\\frac{e^{h}-1}{h}=1$ No.2:**\n","\n","According to L'Hôpital's rule, $\\lim_{x\\to c}\\frac{f(x)}{g(x)}=\\lim_{x\\to c}\\frac{f'(x)}{g'(x)}$\n","\n","$\\therefore\\lim_{h \\to 0}\\frac{e^{h}-1}{h}=\\lim_{h \\to 0}\\frac{e^{h}-0}{1}=\\frac{e^{0}-0}{1}=1$\n","\n","reference:\n","* https://www.quora.com/How-lim-of-h-approach-to-zero-e-h-1-h-is-equal-to-1-but-by-direct-substituting-you-get-0-0"],"metadata":{"id":"jFc5tgP0gQio"}},{"cell_type":"markdown","source":["**Prove that $\\lim_{h\\to0}\\frac{c^{h}-1}{h}=\\log_e(c)=\\ln(c)$:**\n","\n","Given that:\n","* $y=c^h-1$\n","\n","$y+1=c^h$\n","\n","$\\ln(y+1)=\\ln(c^h)$\n","\n","According to Logarithm: $\\log_a(x^y)=y*\\log_a(x)=\\log_a(x)*y$\n","\n","$\\therefore\\ln(y+1)=h*\\ln(c)$\n","\n","$\\frac{\\ln(y+1)}{\\ln(c)}=h$\n","\n","Given that:\n","* $y=c^h-1$\n","* $\\frac{\\ln(y+1)}{\\ln(c)}=h$\n","\n","$\\therefore \\frac{c^h-1}{h}=\\frac{y}{\\frac{\\ln(y+1)}{\\ln(c)}}$\n","\n","$\\frac{c^h-1}{h}=\\frac{y}{\\ln(y+1)}*\\ln(c)=\\ln(c)$\n","\n","\n","reference:\n","* https://math.stackexchange.com/questions/331153/proving-that-lim-h-to-0-fracbh-1h-lnb"],"metadata":{"id":"N6JQ6fyedivN"}},{"cell_type":"markdown","source":["**Prove that: $\\frac{d}{dx}[a^x]=a^x*\\ln(a)$**\n","\n","$\\frac{d}{dx}[a^x]=\\lim_{h\\to0}\\frac{a^{x+h}-a^x}{h}$\n","\n","$\\frac{d}{dx}[a^x]=\\lim_{h\\to0}a^x\\frac{a^{h}-1}{h}$\n","\n","Given that: $\\frac{c^h-1}{h}=\\ln(c)$\n","\n","$\\therefore\\frac{d}{dx}[a^x]=\\lim_{h\\to0}a^x\\ln(a)$"],"metadata":{"id":"s5CFjf4-LVSU"}},{"cell_type":"markdown","source":["###(5) Product Rule, $\\frac{d}{dx}[f(x)*g(x)] = f'(x)*g(x)+g'(x)*f(x)$"],"metadata":{"id":"tFUskp69UuJe"}},{"cell_type":"markdown","source":["$\\frac{d}{dx}[f(x)*g(x)] = f'(x)*g(x)+g'(x)*f(x)$"],"metadata":{"id":"ru5HgNfuVUwd"}},{"cell_type":"markdown","source":["Prove:\n","\n","$z(x)=f(x)*g(x)$\n","\n","$z'(x)= \\lim_{h\\to 0} \\frac{f(x+h)*g(x+h)-f(x)*g(x)}{h}$\n","\n","$z'(x)= \\lim_{h\\to 0} \\frac{f(x+h)*g(x+h)-f(x)*g(x)+f(x+h)*g(x)-f(x+h)*g(x)}{h}$\n","\n","$z'(x)= \\lim_{h\\to 0} \\frac{f(x+h)*g(x+h)-f(x+h)*g(x)-f(x)*g(x)+f(x+h)*g(x)}{h}$\n","\n","$z'(x)= \\lim_{h\\to 0} \\frac{f(x+h)*(g(x+h)-g(x))+g(x)*(f(x+h)-f(x))}{h}$\n","\n","$z'(x)= \\lim_{h\\to 0} \\frac{f(x+h)*(g(x+h)-g(x))}{h}+\\lim_{h\\to 0} \\frac{g(x)*(f(x+h)-f(x))}{h}$\n","\n","$z'(x)= \\lim_{h\\to 0}f(x+h)*\\lim_{h\\to 0} \\frac{(g(x+h)-g(x))}{h}+\\lim_{h\\to 0}g(x)*\\lim_{h\\to 0} \\frac{(f(x+h)-f(x))}{h}$\n","\n","$\\therefore z'(x)= f(x)*g'(x)+g(x)*f'(x)$\n"],"metadata":{"id":"nIqoKB1iVVJe"}},{"cell_type":"markdown","source":["reference:\n","\n","* https://www.khanacademy.org/math/ap-calculus-ab/ab-differentiation-1-new/ab-2-8/a/product-rule-review\n","* https://www.khanacademy.org/math/ap-calculus-ab/ab-differentiation-1-new/ab-diff-1-optional/v/product-rule-proof"],"metadata":{"id":"bzHC1iKfVXBT"}},{"cell_type":"markdown","source":["###(6) Quotient Rule, $\\frac{d}{dx}[\\frac{f(x)}{g(x)}] = \\frac{\\frac{d}{dx}f(x)*g(x)-\\frac{d}{dx}g(x)*f(x)}{(g(x))^2}$"],"metadata":{"id":"68lYTFD0T63X"}},{"cell_type":"markdown","source":["$\\frac{d}{dx}[\\frac{f(x)}{g(x)}] = \\frac{\\frac{d}{dx}f(x)*g(x)-\\frac{d}{dx}g(x)*f(x)}{(g(x))^2}$"],"metadata":{"id":"HHP-J96jmMbe"}},{"cell_type":"markdown","source":["Prove:\n","\n","$f(x) = \\frac{u(x)}{v(x)}$\n","\n","$f'(x) = \\lim_{h\\to 0} \\frac{\\frac{u(x+h)}{v(x+h)}-\\frac{u(x)}{v(x)}}{h}$\n","\n","$= \\lim_{h\\to 0} \\frac{u(x+h)*v(x)-u(x)v(x+h)}{v(x+h)*v(x)*h}$\n","\n","$= \\lim_{h\\to 0} \\frac{u(x+h)*v(x)-u(x)v(x+h)+u(x)*v(x)-u(x)*v(x)}{v(x+h)*v(x)*h}$\n","\n","$= \\lim_{h\\to 0} \\frac{u(x+h)*v(x)-u(x)*v(x)-u(x)v(x+h)+u(x)*v(x)}{v(x+h)*v(x)*h}$\n","\n","$= \\lim_{h\\to 0} \\frac{(u(x+h)-u(x))*v(x)-u(x)(v(x+h)-v(x))}{v(x+h)*v(x)*h}$\n","\n","$= \\lim_{h\\to 0} \\frac{\\frac{(u(x+h)-u(x))}{h}*v(x)-u(x)\\frac{(v(x+h)-v(x))}{h}}{v(x+h)*v(x)}$\n","\n","$\\therefore f'(x) = \\frac{dx}{dy}[\\frac{u'(x)}{v'(x)}]=\\frac{u'(x)*v(x)-v'(x)*u(x)}{(v(x))^2}$"],"metadata":{"id":"1EfjsqDPmNXp"}},{"cell_type":"markdown","source":["###(7) Reciprocal Rule, $\\frac {dy}{dx}[\\frac {1}{f(x)}] = \\frac {-f'(x)}{(f(x))^2}$"],"metadata":{"id":"WYrG-2fT5cWx"}},{"cell_type":"markdown","source":["Prove:\n","\n","$z(x)=\\frac {1}{f(x)}$\n","\n","$z'(x)= \\lim_{h\\to 0} \\frac{\\frac {1}{f(x+h)}-\\frac {1}{f(x)}}{h}$\n","\n","$z'(x)= \\lim_{h\\to 0} \\frac{\\frac {f(x)}{f(x+h)f(x)}-\\frac {f(x+h)}{f(x)f(x+h)}}{h}$\n","\n","$z'(x)= \\lim_{h\\to 0} \\frac{f(x)-f(x+h)}{h*f(x+h)f(x)}$\n","\n","$z'(x)= \\lim_{h\\to 0} \\frac{-(f(x+h)-f(x))}{h*f(x+h)f(x)}$\n","\n","$z'(x)= \\lim_{h\\to 0} \\frac{1}{f(x+h)f(x)}*\\lim_{h\\to 0} \\frac{-(f(x+h)-f(x))}{h}$\n","\n","$z'(x)= \\frac{1}{(f(x))^2}*-1*f'(x)$\n","\n","$\\therefore z'(x)= \\frac{-f'(x)}{(f(x))^2}$"],"metadata":{"id":"U4TbLn2_5_XV"}},{"cell_type":"markdown","source":["###(8) Chain Rule: $\\frac{d}{dx}[f(g(x))] = (f\\circ g)'= f'(g(x))*g'(x)$"],"metadata":{"id":"Vo7n_5EZFt91"}},{"cell_type":"markdown","source":["Composite Function \n","\n","$(f\\circ g) = f(g(x))$\n","\n","$f(x)$ is outer function\n","\n","$g(x)$ is inner function"],"metadata":{"id":"q7XgE4GUd3Sd"}},{"cell_type":"markdown","source":["Example No.1\n","\n","$f(x)=cos(x^2)$\n","\n","$f(x) = cos(x)$ is outer function\n","\n","$g(x) = x^2$ is inner function\n","\n","Example No.2\n","\n","$f(x) = 2x+4$\n","\n","$g(x) = x^3$\n","\n","$(f ∘ g)(x) = f(g(x)) = f(x^3) = 2x^3 + 4$\n","\n","$(g ∘ f)(x) = g(f(x)) = g(2x + 4) = (2x + 4)^3.$"],"metadata":{"id":"VvQsG6U1w6DN"}},{"cell_type":"markdown","source":["Chain Rule\n","\n","$\\frac{d}{dx}[f(g(x))] = f'(g(x))*g'(x)$\n","\n","$\\frac{d}{dx}[f(g(x))] = \\frac{df}{dx}f(g(x)) = \\frac{df}{dg}f(g(x))*\\frac{dg}{dx}g(x)$"],"metadata":{"id":"6PQ0ESKYdx75"}},{"cell_type":"markdown","source":["Note\n","\n","$\\frac{dy}{dx}[f(g(x))] \\neq f'(g(x))$\n","\n","$\\frac{dy}{dx}[f(g(x))] \\neq f'(g'(x))$\n","\n","$\\frac{dy}{dg}f(g(x)) = f'(g(x))*g'(x)$"],"metadata":{"id":"7oTs2cUhILQH"}},{"cell_type":"markdown","source":["Prove: $\\frac{dy}{dg}f(g(x)) = f'(g(x))*g'(x)$\n","\n","$z=f(g(x))$\n","\n","$z'(x) = \\lim_{h\\to 0} \\frac{f(g(x+h))-f(g(x))}{h}$\n","\n","$= \\lim_{h\\to 0} \\frac{f(g(x+h))-f(g(x))}{h}*\\frac{g(x+h)-g(x)}{g(x+h)-g(x)}$\n","\n","$= \\lim_{h\\to 0} \\frac{f(g(x+h))-f(g(x))}{g(x+h)-g(x)}*\\frac{g(x+h)-g(x)}{h}$\n","\n","$= \\lim_{h\\to 0} \\frac{f(g(x+h))-f(g(x))}{g(x+h)-g(x)}*\\lim_{h\\to 0} \\frac{g(x+h)-g(x)}{h}$\n","\n","$= \\lim_{h\\to 0} \\frac{f(g(x+h))-f(g(x))}{g(x+h)-g(x)}*g'(x)$\n","\n","Let $k = g(x+h)-g(x)$\n","\n","$\\therefore g(x+h)=k+g(x)$\n","\n","$z'(x) = \\lim_{k\\to 0} \\frac{f(g(x)+k)-f(g(x))}{k}*g'(x)$\n","\n","$\\therefore z'(x) = \\frac{d}{dx}[f(g(x))]= f'(g(x))*g'(x)$\n","\n"],"metadata":{"id":"gsrsm1vxv2Tg"}},{"cell_type":"markdown","source":["reference\n","* https://tutorial.math.lamar.edu/classes/calci/DerivativeProofs.aspx\n","* https://www.khanacademy.org/math/ap-calculus-ab/ab-differentiation-2-new/ab-diff-2-optional/v/chain-rule-proof\n","* https://www.khanacademy.org/math/ap-calculus-ab/ab-differentiation-2-new/ab-3-1a/a/chain-rule-review\n","* https://youtu.be/m0LZX19DyyI"],"metadata":{"id":"93shqmTUZe4P"}},{"cell_type":"markdown","source":["###Reference"],"metadata":{"id":"I5JR6I4O9wLI"}},{"cell_type":"markdown","source":["reference\n","* https://youtu.be/HfACrKJ_Y2w\n","* https://www.khanacademy.org/math/calculus-1/cs1-derivatives-definition-and-basic-rules/cs1-power-rule/a/justifying-the-power-rule\n","* https://math.stackexchange.com/questions/81325/why-is-xhn-written-like-this\n","* (Prove in Cauculus1) https://tutorial.math.lamar.edu/classes/calci/DerivativeProofs.aspx"],"metadata":{"id":"RHivlJ_1w8Nk"}}]}