{"nbformat":4,"nbformat_minor":0,"metadata":{"colab":{"provenance":[],"authorship_tag":"ABX9TyM+mU3e4eBD1lI0jLmz2ZBP"},"kernelspec":{"name":"python3","display_name":"Python 3"},"language_info":{"name":"python"}},"cells":[{"cell_type":"markdown","source":["###(1) $\\frac{d}{dx}[\\log_a(x)]=\\frac{1}{\\ln(a)*x}$"],"metadata":{"id":"8Hi-CNuL9jZu"}},{"cell_type":"markdown","source":["**Prove that $\\frac{d}{dx}\\log_a(x)=\\frac{1}{x*\\ln(a)}$ No.1:**\n","\n","According to derivative: $\\frac{d}{dx}[f(x)]=\\lim_{h\\to0}\\frac{f(x+h)-f(x)}{h}$\n","\n","$\\frac{d}{dx}[\\log_a(x)]=\\lim_{h\\to0}\\frac{\\log_a(x+h)-\\log_a(x)}{h}$\n","\n","According to Logarithm: $\\log_a(\\frac{x}{y})=\\log_a(x)-\\log_a(y)$\n","\n","$\\frac{d}{dx}[\\log_a(x)]=\\lim_{h\\to0}\\frac{\\log_a(\\frac{x+h}{x})}{h}$\n","\n","$\\frac{d}{dx}[\\log_a(x)]=\\lim_{h\\to0}\\frac{\\log_a(1+\\frac{h}{x})}{h}$\n","\n","Given that:\n","* $\\frac{h}{x}=t\\implies h=xt$\n","* $\\lim_{h\\to0}\\frac{h}{x}=\\lim_{t\\to0}t$\n","\n","$\\therefore\\frac{d}{dx}[\\log_a(x)]=\\lim_{t\\to0}\\frac{\\log_a(1+t)}{xt}$\n","\n","$\\frac{d}{dx}[\\log_a(x)]=\\frac{1}{xt}*\\lim_{t\\to0}\\log_a(1+t)$\n","\n","According to Logarithm: $\\log_a(x^y)=y*\\log_a(x)=\\log_a(x)*y$\n","\n","$\\therefore\\frac{d}{dx}[\\log_a(x)]=\\frac{1}{x}*\\lim_{t\\to0}\\log_a((1+t)^{\\frac{1}{t}})$\n","\n","$\\frac{d}{dx}[\\log_a(x)]=\\frac{1}{x}\\log_a(\\lim_{t\\to0}(1+t)^{\\frac{1}{t}})$\n","\n","According to $e$: $e=\\lim_{n\\to\\infty}(1+\\frac{1}{n})^n=\\lim_{n\\to0}(1+n)^{\\frac{1}{n}}$\n","\n","$\\therefore\\frac{d}{dx}[\\log_a(x)]=\\frac{1}{x}*\\log_a(e)$\n","\n","According to logarithm: $\\log_ac=\\frac{1}{\\log_ca}$\n","\n","$\\therefore\\frac{d}{dx}[\\log_a(x)]=\\frac{1}{x*\\ln(a)}$\n","\n","reference:\n","* https://www.cuemath.com/calculus/derivative-of-log-x/"],"metadata":{"id":"QbCeF0wyeuMN"}},{"cell_type":"markdown","source":["**Find $\\frac{d}{dx}[\\log_af(x)]=?$**"],"metadata":{"id":"xi3szD5Uh-5i"}},{"cell_type":"code","execution_count":null,"metadata":{"id":"SS4pbhmPkgMT"},"outputs":[],"source":[]},{"cell_type":"markdown","source":["###(-2) $\\frac{d}{dx}[f(x)^{g(x)}]$"],"metadata":{"id":"jq26MIQKZa1T"}},{"cell_type":"markdown","source":["reference: https://youtu.be/SUxcFxM65Ho"],"metadata":{"id":"aBnrfP-TZi8v"}},{"cell_type":"markdown","source":["###(-3) $\\frac{d}{dx}[\\log_x(a)]$"],"metadata":{"id":"atoPHEdzlTZx"}}]}