{"nbformat":4,"nbformat_minor":0,"metadata":{"colab":{"provenance":[],"collapsed_sections":["U1AQsJV-ehGw","_geusCTKw0pT","HLh6U2yywxEV","F1ZRSksg2wBY","MMJ5ViiojjVE"],"authorship_tag":"ABX9TyNIvKTSznNoQcQfcXvE/o1R"},"kernelspec":{"name":"python3","display_name":"Python 3"},"language_info":{"name":"python"}},"cells":[{"cell_type":"markdown","source":["###(1) $a^b=c \\implies \\log_ac=b$"],"metadata":{"id":"U1AQsJV-ehGw"}},{"cell_type":"markdown","source":["Types of $\\log_ab$\n","1. Logarithm = $\\log_ab$\n","2. Common Logarithm = $\\log_{10}b=\\log b$\n","3. Natural Logarithm = $\\log_eb=\\ln b$"],"metadata":{"id":"gulV-qn9g9ta"}},{"cell_type":"markdown","source":["Properties\n","* $\\log_ab > 0$\n","* $\\log_aa^x=x$\n","* $a^{\\log_ax}=x$\n","* $\\log_a1=0$"],"metadata":{"id":"N0osngf_wq4H"}},{"cell_type":"markdown","source":["Property of $f(x)=\\log_a(mx+c)$\n","\n","1. Domain (the domain of a function is the set of inputs accepted by the function.)\n","\n","* $mx+c>0$\n","\n","$mx>-c$\n","\n","* If $m>0 \\implies x>\\frac{-c}{|m|} \\therefore$ Domain = $(\\frac{-c}{|m|},\\infty)$\n","\n","* If $m<0 \\implies x<\\frac{-c}{-|m|} \\implies x<\\frac{c}{|m|}$ Domain = $(-\\infty, \\frac{c}{|m|})$\n","\n","2. Range = the difference between the largest and smallest value of $f(x)$. \n","\n","* In this case, range = $(-\\infty,\\infty)$\n","\n","3. Asymptote = a line or curve that acts as the limit of another line or curve. \n","\n","* Horizontal Asymptote = $\\infty$\\\n","\n","* If $m>0 \\implies$ Vertical Asymptote = $\\frac{-c}{|m|}$\n","\n","* If $m<0 \\implies$ Vertical Asymptote = $\\frac{c}{|m|}$"],"metadata":{"id":"kqWZH0tAkugz"}},{"cell_type":"markdown","source":["Example:\n","* $\\log_216=4$\n","* $\\log_381=4$\n","* $\\log_{10}-100=$ Undefined.\n","* $\\log_70=$ Undefined.\n","* etc."],"metadata":{"id":"vvurHEExf1t0"}},{"cell_type":"markdown","source":["###(2) Rules of $\\log$"],"metadata":{"id":"_geusCTKw0pT"}},{"cell_type":"markdown","source":["**Exponential Rules**\n","* $a^0=1$\n","* $a^m*a^n=a^{m+n}$\n","* $\\frac{a^m}{a^n}=a^m*a^{-n}=a^{m-n}$\n","* $(a^m)^n=a^{m*n}$"],"metadata":{"id":"2kshkzsrw6YX"}},{"cell_type":"markdown","source":["**Logarithm Rules**\n","* $\\log_a(1)=0$\n","* $\\log_a(xy)=\\log_a(x)+\\log_a(y)$\n","* $\\log_a(\\frac{x}{y})=\\log_a(x)-\\log_a(y)$\n","* $\\log_a(x^y)=y*\\log_a(x)=\\log_a(x)*y$\n","* $\\log_ab=\\frac{1}{\\log_ba}$"],"metadata":{"id":"xULg-PqfyCEA"}},{"cell_type":"markdown","source":["**Prove that $\\log_a(xy)=\\log_a(x)+\\log_a(y)$:**\n","\n","Let \n","* $x_u=\\log_a(x) \\therefore a^{x_u}=x$\n","* $y_u=\\log_a(y) \\therefore a^{y_u}=y$\n","* $b=\\log_a(\\frac{x}{y})$\n","\n","$a^{b}=xy=a^{x_u}*a^{y_u}=a^{x_u+y_u}$\n","\n","$\\therefore b=x_u+y_u=\\log_a(xy)=\\log_a(x)+\\log_a(y)$\n","\n","reference: https://math.stackexchange.com/questions/2002721/proof-of-logxy-log-x-log-y"],"metadata":{"id":"c9yNa8Xz5qRJ"}},{"cell_type":"markdown","source":["**Prove that $\\log_a(\\frac{x}{y})=\\log_a(x)-\\log_a(y)$:**\n","\n","Let \n","* $x_u=\\log_a(x) \\therefore a^{x_u}=x$\n","* $y_u=\\log_a(y) \\therefore a^{y_u}=y$\n","* $b=\\log_a(\\frac{x}{y})$\n","\n","$a^b=\\frac{x}{y}=\\frac{a^{x_u}}{a^{y_u}}=a^{x_u-y_u}$\n","\n","$\\therefore b = x_u-y_u = \\log_a(\\frac{x}{y})=\\log_a(x)-\\log_a(y)$"],"metadata":{"id":"gHkotCUX-ykX"}},{"cell_type":"markdown","source":["**Prove that $\\log_a(x^y)=y*\\log_a(x)=\\log_a(x)*y$:**\n","\n","Let \n","* $x_u=\\log_a(x) \\therefore a^{x_u}=x$\n","\n","$(a^{x_u})^n=a^{x_u*n}=x^n$\n","\n","$\\therefore \\log_a(x^n)=x_u*n=\\log_a(x)*n$"],"metadata":{"id":"pqI7uNtB_8KP"}},{"cell_type":"markdown","source":["**Prove that: $\\log_ab=\\frac{1}{\\log_ba}$**\n","\n","Given that:\n","* $a^b=c\\implies\\log_ac=b$\n","\n","$a=c^\\frac{1}{b}$\n","\n","$\\therefore\\log_ca=\\frac{1}{b}=\\frac{1}{\\log_ac}$"],"metadata":{"id":"nDy8CuJ6qaQX"}},{"cell_type":"markdown","source":["###(-3) $\\frac{d}{dx}[e^x] =e^x$"],"metadata":{"id":"HLh6U2yywxEV"}},{"cell_type":"markdown","source":["Property $e$\n","\n","1. $\\lim_{n \\to \\infty}(1+\\frac{1}{n})^n=e$\n","2. $\\lim_{h \\to 0}\\frac{e^{h}-1}{h}=1$\n","3. $\\frac{d}{dx}[e^x] = \\lim_{h \\to 0}\\frac{e^{x+h}-e^x}{h} = e^x\\lim_{h \\to 0}\\frac{e^{h}-1}{h} = e^x$"],"metadata":{"id":"5F35d7Gqw28x"}},{"cell_type":"markdown","source":["**Example No1:**\n","\n","$\\frac{d}{dx}[c^x]=\\lim_{h\\to0}\\frac{c^{x+h}-c^x}{h}$\n","\n","$=c^x*\\lim_{h\\to0}\\frac{c^{h}-1}{h}$\n","\n","$=c^x*\\ln(c)$"],"metadata":{"id":"zU4v3_-NI6BV"}},{"cell_type":"markdown","source":["**Prove that $\\lim_{h \\to 0}\\frac{e^{h}-1}{h}=1$**\n","\n","Given that\n","* $y=e^h-1$\n","\n","$\\therefore y+1=e^h$\n","\n","$\\log_e(y+1)=\\log_e(e^h)$\n","\n","According to Logarithm property: $\\log_aa^x=x$\n","\n","$\\therefore \\log_e(y+1)=h$\n","\n","Given that\n","* $y=e^h-1$\n","* $\\log_e(y+1)=h$\n","\n","$\\therefore \\frac{e^{h}-1}{h}=\\frac{y}{\\log_e(y+1)}=\\frac{e^{h}-1}{\\log_e(e^h-1+1)}$\n","\n","Given that:\n","* $\\lim_{h\\to0}e^h-1=\\lim_{y\\to0}y$\n","\n","$\\therefore \\lim_{h\\to0}\\frac{e^{h}-1}{h}=\\lim_{y\\to0}\\frac{y}{\\log_e(y+1)}$\n","\n","$\\lim_{y\\to0}\\frac{y}{\\ln(y+1)}=\\lim_{y\\to0}\\frac{1}{\\frac{\\ln(y+1)}{y}}$\n","\n","$\\lim_{y\\to0}\\frac{y}{\\ln(y+1)}=\\lim_{y\\to0}\\frac{1}{\\frac{1}{y}*\\ln(y+1)}$\n","\n","\n","According to Logarithm property: $\\log_a(x^y)=y*\\log_a(x)=\\log_a(x)*y$\n","\n","$\\therefore\\lim_{y\\to0}\\frac{y}{\\ln(y+1)}=\\lim_{y\\to0}\\frac{1}{\\ln((y+1)^\\frac{1}{y})}$\n","\n","Given that\n","* $\\lim_{n\\to\\infty}(1+\\frac{1}{n})^n=e$\n","* $\\lim_{n\\to\\infty}\\frac{1}{n}=\\lim_{y\\to0}y$\n","* $\\therefore \\lim_{n\\to\\infty}(1+\\frac{1}{n})^n=\\lim_{y\\to0}(y+1)^\\frac{1}{y}=e$\n","\n","$\\therefore\\lim_{y\\to0}\\frac{y}{\\ln(y+1)}=\\frac{1}{\\ln(e)}$\n","\n","According to Logarithm property: $\\log_aa^x=x$\n","\n","$\\therefore\\lim_{y\\to0}\\frac{y}{\\ln(y+1)}=\\frac{1}{1}=1$\n","\n","reference:\n","* https://youtu.be/qWw8VnzTddg\n","* https://socratic.org/questions/how-do-you-solve-the-following-limit-e-x-1-x-as-x-approaches-zero"],"metadata":{"id":"7rJUQgU0Xohu"}},{"cell_type":"markdown","source":["**Prove that $\\lim_{h \\to 0}\\frac{e^{h}-1}{h}=1$ No.2**\n","\n","According to L'HÃ´pital's rule, $\\lim_{x\\to c}\\frac{f(x)}{g(x)}=\\lim_{x\\to c}\\frac{f'(x)}{g'(x)}$\n","\n","$\\therefore\\lim_{h \\to 0}\\frac{e^{h}-1}{h}=\\lim_{h \\to 0}\\frac{e^{h}-0}{1}=\\frac{e^{0}-0}{1}=1$\n","\n","reference:\n","* https://www.quora.com/How-lim-of-h-approach-to-zero-e-h-1-h-is-equal-to-1-but-by-direct-substituting-you-get-0-0"],"metadata":{"id":"jFc5tgP0gQio"}},{"cell_type":"markdown","source":["**Unfinished, Prove that $\\lim_{h \\to 0}\\frac{e^{h}-1}{h}=1$ No.3**\n","\n","???\n","\n","reference:\n","* https://math.stackexchange.com/questions/2832934/how-to-prove-that-lim-h-to-0-fraceh-1h"],"metadata":{"id":"wjv0FtUkk8qJ"}},{"cell_type":"markdown","source":["**Prove that $\\lim_{h\\to0}\\frac{c^{h}-1}{h}=\\log_e(c)=\\ln(c)$: No.1**\n","\n","Given that:\n","* $y=c^h-1$\n","\n","$\\lim_{y\\to0}y+1=\\lim_{h\\to0}c^h$\n","\n","$y+1=c^h$\n","\n","$\\ln(y+1)=\\ln(c^h)$\n","\n","According to Logarithm: $\\log_a(x^y)=y*\\log_a(x)=\\log_a(x)*y$\n","\n","$\\therefore\\ln(y+1)=h*\\ln(c)$\n","\n","$\\frac{\\ln(y+1)}{\\ln(c)}=h$\n","\n","Given that:\n","* $y=c^h-1$\n","* $\\frac{\\ln(y+1)}{\\ln(c)}=h$\n","\n","$\\therefore \\frac{c^h-1}{h}=\\frac{y}{\\frac{\\ln(y+1)}{\\ln(c)}}$\n","\n","$\\frac{c^h-1}{h}=\\frac{y}{\\ln(y+1)}*\\ln(c)$\n","\n","$\\frac{c^h-1}{h}=\\frac{1}{\\frac{1}{y}*\\ln(y+1)}*\\ln(c)$\n","\n","According to Logarithm property: $\\log_a(x^y)=y*\\log_a(x)=\\log_a(x)*y$\n","\n","$\\frac{c^h-1}{h}=\\frac{1}{\\ln((y+1)^{\\frac{1}{y}})}*\\ln(c)$\n","\n","Given that\n","* $\\lim_{n\\to\\infty}(1+\\frac{1}{n})^n=e$\n","* $\\lim_{n\\to\\infty}\\frac{1}{n}=\\lim_{y\\to0}y$\n","* $\\therefore \\lim_{n\\to\\infty}(1+\\frac{1}{n})^n=\\lim_{y\\to0}(y+1)^\\frac{1}{y}=e$\n","\n","$\\therefore\\frac{c^h-1}{h}=\\frac{1}{\\ln(e))}*\\ln(c)$\n","\n","According to Logarithm property: $\\log_aa^x=x$\n","\n","$\\therefore\\frac{c^h-1}{h}=\\ln(c)$\n","\n","\n","reference:\n","* https://math.stackexchange.com/questions/331153/proving-that-lim-h-to-0-fracbh-1h-lnb"],"metadata":{"id":"N6JQ6fyedivN"}},{"cell_type":"markdown","source":["###(-4) $e=\\Sigma_{k=0}^{\\infty}\\frac{1}{k!}$"],"metadata":{"id":"MMJ5ViiojjVE"}},{"cell_type":"markdown","source":["**Proof No.1: (Unfinished)**\n","\n","Given that:\n","* $e=\\lim_{k\\to\\infty}(1+\\frac{1}{k})^k$\n","\n","According to Binomial theorem: $(x+y)^n=\\Sigma_{r=0}^n\\frac{n!}{(n-r)!*r!}x^{n-r}y^r$\n","\n","$\\therefore e=\\lim_{k\\to\\infty}(1+\\frac{1}{k})^k=\\lim_{k\\to\\infty}\\Sigma_{r=0}^k\\frac{k!}{(k-r)!*r!}1^{k-r}*(\\frac{1}{k})^r$\n","\n","$e=\\lim_{k\\to\\infty}(1+\\frac{1}{k})^k=\\lim_{k\\to\\infty}\\Sigma_{r=0}^k\\frac{k!}{(k-r)!*r!}(\\frac{1}{k})^r$\n","\n","$e=\\lim_{k\\to\\infty}(1+\\frac{1}{k})^k=\\lim_{k\\to\\infty}\\Sigma_{r=0}^k\\frac{k!}{(k-r)!*r!}*k^{-r}$\n","\n","$e=\\lim_{k\\to\\infty}(1+\\frac{1}{k})^k=\\lim_{k\\to\\infty}\\Sigma_{r=0}^k\\frac{(k-1)!}{(k-r)!*r!}k^{-r+1}$\n","\n","\n","Note:\n","\n","$e=\\lim_{k\\to\\infty}(1+\\frac{1}{k})^k=\\lim_{k\\to\\infty}\\Sigma_{r=0}^k\\frac{k*(k-1)*...*(k-r+1)*(k-r)*(k-r-1)*...*(1)}{(k-r)*(k-r-1)*...*(1)*r*(r-1)*...*(1)}(\\frac{1}{k})^r$\n","\n","$\\therefore e=\\lim_{k\\to\\infty}(1+\\frac{1}{k})^k=\\lim_{k\\to\\infty}\\Sigma_{r=0}^k\\frac{k*(k-1)*...*(k-r+1)}{r*(r-1)*...*(1)}(\\frac{1}{k})^r$\n","\n","$\\therefore e=\\lim_{k\\to\\infty}(1+\\frac{1}{k})^k=\\lim_{k\\to\\infty}\\Sigma_{r=0}^k\\frac{(k-1)*...*(k-r+1)}{r*(r-1)*...*(1)}(\\frac{1}{k})^{r-1}$\n","\n","if\n","1. $r=0\\implies \\lim_{k\\to\\infty} \\frac{k!}{k!}*k^{0} = 1$\n","1. $r=1\\implies \\lim_{k\\to\\infty} \\frac{k!}{(k-1)!}*k^{-1} = 1$\n","1. $r=2\\implies \\lim_{k\\to\\infty} \\frac{k!}{(k-2)!*2}*k^{-2}$\n","* $\\therefore lim_{k\\to\\infty} \\frac{k!}{(k-2)!*2}*k^{-2}= lim_{k\\to\\infty} \\frac{(k-1)!}{(k-2)!*2}*k^{-1}$\n","* $\\therefore lim_{k\\to\\infty} \\frac{k!}{(k-2)!*2}*k^{-2}= lim_{k\\to\\infty} \\frac{(k-1)!}{k*(k-2)!*2}$\n","* $\\therefore lim_{k\\to\\infty} \\frac{k!}{(k-2)!*2}*k^{-2}c= lim_{k\\to\\infty} \\frac{(k-1)}{k*2}$\n","* $\\therefore lim_{k\\to\\infty} \\frac{k!}{(k-2)!*2}*k^{-2}c= lim_{k\\to\\infty} \\frac{(k-1)}{k}*\\frac{1}{2}$\n","* $\\therefore lim_{k\\to\\infty} \\frac{k!}{(k-2)!*2}*k^{-2}c\n","= \\frac{1}{2}$\n","1. $r=3\\implies \\lim_{k\\to\\infty} \\frac{k!}{(k-3)!*3!}*k^{-3} = 1$\n","\n","\n","$e=\\lim_{k\\to\\infty}(1+\\frac{1}{k})^k=\\lim_{k\\to\\infty}\\Sigma_{r=0}^k\\frac{k*(k-1)*...*1}{(k-r)*(k-r-1)*...*(1)*r*(r-1)*...*(1)}(\\frac{1}{k})*(\\frac{1}{k})*...*(\\frac{1}{k})$\n","\n","\n","$r\\leq k$"],"metadata":{"id":"rinxe5nhkzBu"}},{"cell_type":"markdown","source":["**Proof No.2: (Unfinished)**\n","\n","\n","Given that:\n","* $e=\\lim_{k\\to\\infty}(1+\\frac{1}{k})^k$\n","* $e=\\Sigma_{k=0}^{\\infty}\\frac{1}{k!}$\n","\n","According to Binomial theorem: $(x+y)^n=\\Sigma_{r=0}^n\\frac{n!}{(n-r)!*r!}x^{n-r}y^r$\n","\n","$\\therefore e=\\lim_{k\\to\\infty}(1+\\frac{1}{k})^k=\\lim_{k\\to\\infty}\\Sigma_{r=0}^k\\frac{k!}{(k-r)!*r!}1^{k-r}*(\\frac{1}{k})^r$\n","\n","$e=\\lim_{k\\to\\infty}(1+\\frac{1}{k})^k=\\lim_{k\\to\\infty}\\Sigma_{r=0}^k\\frac{k!}{(k-r)!*r!}(\\frac{1}{k})^r$\n","\n","$e=\\lim_{k\\to\\infty}(1+\\frac{1}{k})^k=\\lim_{k\\to\\infty}\\Sigma_{r=0}^k\\frac{k!}{(k-r)!*r!}*k^{-r}$\n","\n","$\\therefore e=\\lim_{n\\to\\infty}\\Sigma_{k=0}^n\\frac{n!}{(n-k)!*k!*n}=\\Sigma_{k=0}^{\\infty}\\frac{1}{k!}\\implies \\lim_{n\\to\\infty}\\Sigma_{k=0}^n\\frac{n!}{(n-k)!*n}=1$"],"metadata":{"id":"9iT6MnHPzQl6"}},{"cell_type":"markdown","source":["$e=\\lim_{n\\to\\infty}(1+\\frac{1}{n})^n$"],"metadata":{"id":"7kcuhEhSkRpn"}},{"cell_type":"markdown","source":["reference:\n","* https://en.wikipedia.org/wiki/List_of_representations_of_e#As_an_infinite_series"],"metadata":{"id":"dWnCE4EPv047"}},{"cell_type":"markdown","source":["###(5) $\\frac{d}{dx}c^x=c^x*\\ln(c)$"],"metadata":{"id":"F1ZRSksg2wBY"}},{"cell_type":"markdown","source":["**Prove:**\n","\n","$\\frac{d}{dx}c^x=\\lim_{h\\to0}\\frac{c^{x+h}-c^x}{h}$\n","\n","$\\frac{d}{dx}c^x=c^x*\\lim_{h\\to0}\\frac{c^{h}-1}{h}$\n","\n","Given that: \n","* $\\lim_{h\\to0}\\frac{c^{h}-1}{h}=\\ln(c)$\n","\n","$\\therefore\\frac{d}{dx}c^x=c^x*\\ln(c)$"],"metadata":{"id":"oTfzddW14k_8"}},{"cell_type":"markdown","source":["###(6) $\\frac{d}{dx}\\log_a(x)=\\frac{1}{x*\\ln(a)}$"],"metadata":{"id":"00MlsxEW89P9"}},{"cell_type":"markdown","source":["**Prove that $\\frac{d}{dx}\\log_a(x)=\\frac{1}{x*\\ln(a)}$ No.1:**\n","\n","According to derivative: $\\frac{d}{dx}[f(x)]=\\lim_{h\\to0}\\frac{f(x+h)-f(x)}{h}$\n","\n","$\\frac{d}{dx}[\\log_a(x)]=\\lim_{h\\to0}\\frac{\\log_a(x+h)-\\log_a(x)}{h}$\n","\n","According to Logarithm: $\\log_a(\\frac{x}{y})=\\log_a(x)-\\log_a(y)$\n","\n","$\\frac{d}{dx}[\\log_a(x)]=\\lim_{h\\to0}\\frac{\\log_a(\\frac{x+h}{x})}{h}$\n","\n","$\\frac{d}{dx}[\\log_a(x)]=\\lim_{h\\to0}\\frac{\\log_a(1+\\frac{h}{x})}{h}$\n","\n","Given that:\n","* $\\frac{h}{x}=t\\implies h=xt$\n","* $\\lim_{h\\to0}\\frac{h}{x}=\\lim_{t\\to0}t$\n","\n","$\\therefore\\frac{d}{dx}[\\log_a(x)]=\\lim_{t\\to0}\\frac{\\log_a(1+t)}{xt}$\n","\n","$\\frac{d}{dx}[\\log_a(x)]=\\frac{1}{xt}*\\lim_{t\\to0}\\log_a(1+t)$\n","\n","According to Logarithm: $\\log_a(x^y)=y*\\log_a(x)=\\log_a(x)*y$\n","\n","$\\therefore\\frac{d}{dx}[\\log_a(x)]=\\frac{1}{x}*\\lim_{t\\to0}\\log_a((1+t)^{\\frac{1}{t}})$\n","\n","$\\frac{d}{dx}[\\log_a(x)]=\\frac{1}{x}\\log_a(\\lim_{t\\to0}(1+t)^{\\frac{1}{t}})$\n","\n","According to $e$: $e=\\lim_{n\\to\\infty}(1+\\frac{1}{n})^n=\\lim_{n\\to0}(1+n)^{\\frac{1}{n}}$\n","\n","$\\therefore\\frac{d}{dx}[\\log_a(x)]=\\frac{1}{x}*\\log_a(e)$\n","\n","According to logarithm: $\\log_ac=\\frac{1}{\\log_ca}$\n","\n","$\\therefore\\frac{d}{dx}[\\log_a(x)]=\\frac{1}{x*\\ln(a)}$\n","\n","reference:\n","* https://www.cuemath.com/calculus/derivative-of-log-x/"],"metadata":{"id":"QbCeF0wyeuMN"}},{"cell_type":"markdown","source":["**Prove that $\\frac{d}{dx}\\log_a(x)=\\frac{1}{x*\\ln(a)}$ No.2:**\n","\n","According to derivative: $\\frac{d}{dx}[f(x)]=\\lim_{h\\to0}\\frac{f(x+h)-f(x)}{h}$\n","\n","$\\frac{d}{dx}[\\log_a(x)]=\\lim_{h\\to0}\\frac{\\log_a(x+h)-\\log_a(x)}{h}$\n","\n","According to Logarithm: $\\log_a(\\frac{x}{y})=\\log_a(x)-\\log_a(y)$\n","\n","$\\frac{d}{dx}[\\log_a(x)]=\\lim_{h\\to0}\\frac{\\log_a(\\frac{x+h}{x})}{h}$\n","\n","$\\frac{d}{dx}[\\log_a(x)]=\\lim_{h\\to0}\\frac{\\log_a(1+\\frac{h}{x})}{h}$\n","\n","Given that:\n","* $\\lim_{y\\to1}y=\\lim_{h\\to0}1+\\frac{h}{x}\\implies\\lim_{h\\to0} h=\\lim_{y\\to1}x(y-1)$\n","\n","$\\therefore\\frac{d}{dx}[\\log_a(x)]=\\lim_{y\\to1}\\frac{\\log_a(y)}{x(y-1)}$\n","\n","$\\frac{d}{dx}[\\log_a(x)]=\\frac{1}{x}*\\lim_{y\\to1}\\frac{\\log_a(y)}{y-1}$\n","\n","Given that:\n","* $\\lim_{y\\to1}y-1=\\lim_{z\\to0}z\\implies\\lim_{y\\to1}\\log_ay=\\lim_{z\\to0}\\log_a(z+1)$\n","\n","$\\therefore\\frac{d}{dx}[\\log_a(x)]=\\frac{1}{x}*\\lim_{z\\to0}\\frac{\\log_a(z+1)}{z}$\n","\n","According to logarithm: $\\log_a(x^y)=y*\\log_a(x)=\\log_a(x)*y$\n","\n","$\\therefore\\frac{d}{dx}[\\log_a(x)]=\\frac{1}{x}*\\lim_{z\\to0}\\log_a((z+1)^{\\frac{1}{z}})$\n","\n","$\\frac{d}{dx}[\\log_a(x)]=\\frac{1}{x}*\\log_a(\\lim_{z\\to0}(z+1)^{\\frac{1}{z}})$\n","\n","According to $e$: $e=\\lim_{n\\to0}(1+n)^\\frac1n$\n","\n","$\\therefore\\frac{d}{dx}[\\log_a(x)]=\\frac{1}{x}*\\log_a(e)$\n","\n","According to logarithm: $\\log_ab=\\frac{1}{\\log_ba}$\n","\n","$\\therefore\\frac{d}{dx}[\\log_a(x)]=\\frac{1}{x*\\ln(a)}$\n"],"metadata":{"id":"_tPAi92yuB0U"}},{"cell_type":"markdown","source":["###(7) $\\frac{d}{dx}[x^x]$"],"metadata":{"id":"txSPUvd9d-vX"}},{"cell_type":"markdown","source":["Given that: $y=x^x$\n","\n","$\\therefore \\ln(y)=\\ln(x^x)$\n","\n","According to Logarithm: $\\log_a(x^y)=y*\\log_a(x)=\\log_a(x)*y$\n","\n","$\\therefore \\ln(y)=x*\\ln(x)$\n","\n","$\\frac{dy}{dx}[\\ln(y)]=\\frac{dy}{dx}[x*\\ln(x)]$\n","\n","According to Product Rule: $\\frac{d}{dx}[f(x)*g(x)] = f'(x)*g(x)+g'(x)*f(x)$\n","\n","$\\therefore\\frac{dy}{dx}[\\ln(y)]=\\frac{dy}{dx}[x]*\\ln(x)+x*\\frac{dy}{dx}[\\ln(x)]$\n","\n","$\\therefore\\frac{dy}{dx}[\\ln(y)]=\\ln(x)+x*\\frac{dy}{dx}[\\ln(x)]$\n","\n","According to derivertive: $\\frac{d}{dx}[\\log_a(x)]=\\frac{1}{\\ln(a)*x}$\n","\n","Given that: $\\ln(e)=1$\n","\n","$\\therefore\\frac{dy}{dx}[\\ln(y)]=\\ln(x)+x*\\frac{1}{x}$\n","\n","$\\therefore\\frac{dy}{dx}[\\ln(y)]=\\ln(x)+1$\n","\n","According to Chain Rule: $\\frac{d}{dx}[f(g(x))] = (f\\circ g)'= f'(g(x))*g'(x)$\n","\n","Given that:\n","* $f(x)=\\ln(x)\\implies f'(x)=\\frac{1}{x}$\n","* $g(x)=y\\implies g'(x)=\\frac{dy}{dx}$\n","\n","$\\therefore\\frac{1}{y}*\\frac{dy}{dx}=\\ln(x)+1$\n","\n","$\\frac{dy}{dx}=y*(\\ln(x)+1)$\n","\n","Given that: $y=x^x$\n","\n","$\\therefore\\frac{dy}{dx}=x^x*(\\ln(x)+1)$\n"],"metadata":{"id":"GIi4d7jzd-vY"}},{"cell_type":"markdown","source":["###(8) $\\frac{d}{dx}[\\log_a(x)]=\\frac{1}{\\ln(a)*x}$"],"metadata":{"id":"8Hi-CNuL9jZu"}},{"cell_type":"markdown","source":["**Prove that $\\frac{d}{dx}\\log_a(x)=\\frac{1}{x*\\ln(a)}$ No.1:**\n","\n","According to derivative: $\\frac{d}{dx}[f(x)]=\\lim_{h\\to0}\\frac{f(x+h)-f(x)}{h}$\n","\n","$\\frac{d}{dx}[\\log_a(x)]=\\lim_{h\\to0}\\frac{\\log_a(x+h)-\\log_a(x)}{h}$\n","\n","According to Logarithm: $\\log_a(\\frac{x}{y})=\\log_a(x)-\\log_a(y)$\n","\n","$\\frac{d}{dx}[\\log_a(x)]=\\lim_{h\\to0}\\frac{\\log_a(\\frac{x+h}{x})}{h}$\n","\n","$\\frac{d}{dx}[\\log_a(x)]=\\lim_{h\\to0}\\frac{\\log_a(1+\\frac{h}{x})}{h}$\n","\n","Given that:\n","* $\\frac{h}{x}=t\\implies h=xt$\n","* $\\lim_{h\\to0}\\frac{h}{x}=\\lim_{t\\to0}t$\n","\n","$\\therefore\\frac{d}{dx}[\\log_a(x)]=\\lim_{t\\to0}\\frac{\\log_a(1+t)}{xt}$\n","\n","$\\frac{d}{dx}[\\log_a(x)]=\\frac{1}{xt}*\\lim_{t\\to0}\\log_a(1+t)$\n","\n","According to Logarithm: $\\log_a(x^y)=y*\\log_a(x)=\\log_a(x)*y$\n","\n","$\\therefore\\frac{d}{dx}[\\log_a(x)]=\\frac{1}{x}*\\lim_{t\\to0}\\log_a((1+t)^{\\frac{1}{t}})$\n","\n","$\\frac{d}{dx}[\\log_a(x)]=\\frac{1}{x}\\log_a(\\lim_{t\\to0}(1+t)^{\\frac{1}{t}})$\n","\n","According to $e$: $e=\\lim_{n\\to\\infty}(1+\\frac{1}{n})^n=\\lim_{n\\to0}(1+n)^{\\frac{1}{n}}$\n","\n","$\\therefore\\frac{d}{dx}[\\log_a(x)]=\\frac{1}{x}*\\log_a(e)$\n","\n","According to logarithm: $\\log_ac=\\frac{1}{\\log_ca}$\n","\n","$\\therefore\\frac{d}{dx}[\\log_a(x)]=\\frac{1}{x*\\ln(a)}$\n","\n","reference:\n","* https://www.cuemath.com/calculus/derivative-of-log-x/"],"metadata":{"id":"QIT5DX-VkKnH"}},{"cell_type":"markdown","source":["**Find $\\frac{d}{dx}[\\log_af(x)]=?$**"],"metadata":{"id":"xi3szD5Uh-5i"}}]}