{"nbformat":4,"nbformat_minor":0,"metadata":{"colab":{"provenance":[],"authorship_tag":"ABX9TyOXawFMQBY2Ig8pNWG5M1LW"},"kernelspec":{"name":"python3","display_name":"Python 3"},"language_info":{"name":"python"}},"cells":[{"cell_type":"markdown","source":["###(1): $\\frac{d}{dx}[f(x)^{g(x)}]=?$"],"metadata":{"id":"H5tefCzcZej0"}},{"cell_type":"markdown","source":["**Keyword No.1**\n","* $\\frac{d}{dx}[f(x)^{g(x)}]$\n","* $\\lim_{h\\to0}(x+h)^{x+h}$\n","* $\\frac{d}{dx}[x^x]$\n","* $\\frac{d}{dx}[ax^{bx}]$\n","* $\\frac{d}{dx}[(ax+c_a)^{bx+c_b}]$\n","* Fractional Binomial Theorem\n","* Series\n","* Maclaurin Series\n","* Taylor Series"],"metadata":{"id":"_Jgc4CKJe84N"}},{"cell_type":"markdown","source":["**To Do Now**\n","\n","1. $\\frac{d}{dx}[x^x]$\n","* https://socratic.org/questions/d-dx-x-x\n","* https://youtu.be/l-iLg07zavc\n","2. Fractional Binomial Theorem\n","* https://brilliant.org/wiki/fractional-binomial-theorem/\n","\n","**Mathematics Problems No.1**\n","1. $\\frac{d}{dx}[f(x)^{g(x)}]$\n","2. $\\lim_{h\\to0}(x+h)^{x+h}$\n","3. $\\frac{d}{dx}[x^x]$\n","4. $\\frac{d}{dx}[ax^{bx}]$\n","5. $\\frac{d}{dx}[(ax+c_a)^{bx+c_b}]$\n","\n","**Mathematics Problems No.2**\n","6. $\\lim_{k\\to\\infty}\\frac{n!}{(n-k)!*k!}*x^k$\n","7. Proof that: $(x+1)^{\\frac{1}{2}}=f(0)x^0+f'(0)x^1+f''(0)x^2+...+f^{(k)}x^k$\n","8. Proof that: $(x+1)^n=\\Sigma_{k=0}^{\\infty}\\frac{n!}{(n-k)!*k!}*x^k$"],"metadata":{"id":"Uab17X7mxZQm"}},{"cell_type":"markdown","source":["**Example No.1:**\n","\n","Given that:\n","\n","* $f(x)=m_fx$\n","* $g(x)=m_gx$\n","\n","$\\therefore \\frac{d}{dx}[f(x)^{g(x)}]=\\frac{d}{dx}[m_fx^{m_gx}]$\n","\n","Assume that:\n","* $$"],"metadata":{"id":"LwMWRW1lakEL"}},{"cell_type":"markdown","source":["**Example No.2:**\n","\n","Given that:\n","\n","* $f(x)=m_fx+c_f$\n","* $g(x)=m_gx+c_g$\n","\n","$\\therefore \\frac{d}{dx}[f(x)^{g(x)}]=\\frac{d}{dx}[(m_fx+c_f)^{m_gx+c_g}]$\n","\n","Assume that:\n","* $$\n"],"metadata":{"id":"hCWEMnnrZoeI"}},{"cell_type":"markdown","source":[],"metadata":{"id":"ICkmxsn3ahry"}},{"cell_type":"markdown","source":["reference: \n","* https://youtu.be/SUxcFxM65Ho\n","* https://youtu.be/3FI9jn57Oho"],"metadata":{"id":"rjFQIqSqZlbh"}},{"cell_type":"markdown","source":["###(2) $(x+y)^{x+y}=?$"],"metadata":{"id":"BI90VbSMvfSE"}},{"cell_type":"markdown","source":["**Find $(x+y)^{x+y}=?$**\n","\n","According to Binomial theorem: $(x+y)^n=\\Sigma_{r=0}^n\\frac{n!}{(n-r)!*r!}x^{n-r}y^r$\n","\n","$\\therefore(x+y)^{x+y}=\\Sigma_{r=0}^{x+y}\\frac{(x+y)!}{((x+y)-r)!*r!}x^{x+y-r}y^r$"],"metadata":{"id":"-9lmbl700Kgu"}},{"cell_type":"markdown","source":["###(3) $\\frac{d}{dx}[x^x]$"],"metadata":{"id":"e6uAhII4vvbP"}},{"cell_type":"markdown","source":["**Find $\\frac{d}{dx}[x^x]$ Solution No.1**\n","\n","$y=x^x$\n","\n","$\\ln(y)=\\ln(x^x)$\n","\n","According to Logarithm: $\\log_a(x^y)=y*\\log_a(x)=\\log_a(x)*y$\n","\n","$\\therefore\\ln(y)=x*\\ln(x)$\n","\n","$\\frac{dy}{dx}[\\ln(y)]=\\frac{dy}{dx}[x*\\ln(x)]$\n","\n","According to derivative: $\\frac{d}{dx}[\\ln(x)]=\\frac{1}{x}$\n","\n","$\\therefore\\frac{dy}{dx}*\\frac{1}{y}=\\frac{dy}{dx}[x*\\ln(x)]$\n","\n","According to Product Rule, $\\frac{d}{dx}[f(x)*g(x)] = f'(x)*g(x)+g'(x)*f(x)$\n","\n","$\\therefore\\frac{dy}{dx}*\\frac{1}{y}=\\frac{dy}{dx}[x]*\\ln(x)+\\frac{dy}{dx}[\\ln(x)]*x$\n","\n","$\\frac{dy}{dx}*\\frac{1}{y}=\\ln(x)+\\frac{1}{x}*x$\n","\n","$\\frac{dy}{dx}*\\frac{1}{y}=\\ln(x)+1$\n","\n","$\\frac{dy}{dx}=y(\\ln(x)+1)$\n","\n","Given that: $y=x^x$\n","\n","$\\therefore\\frac{dy}{dx}=x^x(\\ln(x)+1)$\n","\n","reference: https://socratic.org/questions/d-dx-x-x"],"metadata":{"id":"NBtxu9ExvxMK"}},{"cell_type":"markdown","source":["**Find $\\frac{d}{dx}[x^x]$ Solution No.2**\n","\n","$\\frac{d}{dx}[x^x]=\\lim_{h\\to0}\\frac{(x+h)^{x+h}-x^x}{h}$\n","\n","According to Binomial theorem: $(x+y)^n=\\Sigma_{r=0}^n\\frac{n!}{(n-r)!*r!}x^{n-r}y^r$\n","\n","$\\therefore\\frac{d}{dx}[x^x]=\\lim_{h\\to0}\\frac{1}{h}*(\\Sigma_{r=0}^{x+h}\\frac{(x+h)!}{(x+h-r)!*r!}x^{x+h-r}h^r-x^x)$\n","\n","$\\frac{d}{dx}[x^x]=\\lim_{h\\to0}\\frac{1}{h}*(x^{x+h}+(x+h)x^{x+h-1}h+\\frac{(x+h)(x+h-1)}{2}x^{x+h-2}h^2+...-x^x)$\n","\n","$\\frac{d}{dx}[x^x]=\\lim_{h\\to0}\\frac{1}{h}*(x^{x+h}-x^x+(x+h)x^{x+h-1}h+\\frac{(x+h)(x+h-1)}{2}x^{x+h-2}h^2+...)$\n","\n","$\\frac{d}{dx}[x^x]=\\lim_{h\\to0}\\frac{x^{x+h}-x^x}{h}+\\lim_{h\\to0}\\frac{1}{h}((x+h)x^{x+h-1}h+\\frac{(x+h)(x+h-1)}{2}x^{x+h-2}h^2+...)$\n","\n","$\\frac{d}{dx}[x^x]=x^x*\\lim_{h\\to0}\\frac{x^{h}-1}{h}+\\lim_{h\\to0}\\frac{1}{h}((x+h)x^{x+h-1}h+\\frac{(x+h)(x+h-1)}{2}x^{x+h-2}h^2+...)$\n","\n","Given that: $\\lim_{h\\to0}\\frac{x^{h}-1}{h}=\\ln(x)$\n","\n","$\\frac{d}{dx}[x^x]=x^x*\\ln(x)+\\lim_{h\\to0}\\frac{1}{h}((x+h)x^{x+h-1}h+\\frac{(x+h)(x+h-1)}{2}x^{x+h-2}h^2+...)$\n","\n","$\\frac{d}{dx}[x^x]=x^x*\\ln(x)+\\lim_{h\\to0}((x+h)x^{x+h-1}+\\frac{(x+h)(x+h-1)}{2}x^{x+h-2}h+...)$\n","\n","$\\frac{d}{dx}[x^x]=x^x*\\ln(x)+\\lim_{h\\to0}((x+h)x^{x+h-1}+h*(\\frac{(x+h)(x+h-1)}{2}x^{x+h-2}+...))$\n","\n","$\\frac{d}{dx}[x^x]=x^x*\\ln(x)+\\lim_{h\\to0}((x+h)x^{x+h-1})$\n","\n","$\\frac{d}{dx}[x^x]=x^x*\\ln(x)+((x)x^{x-1})$\n","\n","$\\therefore\\frac{d}{dx}[x^x]=x^x*\\ln(x)+x^x$\n","\n","Question:\n","* How can Binomial theorem be applied with non-integer power?"],"metadata":{"id":"NiEjZ4Fuv2vo"}},{"cell_type":"markdown","source":["**Find $\\frac{d}{dx}[x^x]$ Solution No.2**\n","\n","$\\frac{d}{dx}[x^x]=\\lim_{h\\to0}\\frac{(x+h)^{x+h}-x^x}{h}$"],"metadata":{"id":"N1OsvF1szqzJ"}},{"cell_type":"markdown","source":["###(4) $\\frac{d}{dx}[(\\Sigma_{i=0}^nc_ix^i)^{\\Sigma_{j=0}^mc_jx^j}]$"],"metadata":{"id":"kehKI2y5EUq1"}},{"cell_type":"markdown","source":["###(5) Find Integral of $x^x$"],"metadata":{"id":"nbTNSz2uEvWb"}},{"cell_type":"markdown","source":["###(6) $\\lim_{h \\to 0}\\frac{e^{h}-1}{h}=1$ and $\\lim_{h \\to 0}\\frac{c^{h}-1}{h}=\\ln(c)$"],"metadata":{"id":"jgfrn56NcPeC"}},{"cell_type":"markdown","source":["**Proof No.1: $\\lim_{h \\to 0}\\frac{e^{h}-1}{h}=1$**\n","\n","Given that\n","* $y=e^h-1$\n","\n","$\\therefore y+1=e^h$\n","\n","$\\log_e(y+1)=\\log_e(e^h)$\n","\n","According to Logarithm property: $\\log_aa^x=x$\n","\n","$\\therefore \\log_e(y+1)=h$\n","\n","Given that\n","* $y=e^h-1$\n","* $\\log_e(y+1)=h$\n","\n","$\\therefore \\frac{e^{h}-1}{h}=\\frac{y}{\\log_e(y+1)}=\\frac{e^{h}-1}{\\log_e(e^h-1+1)}$\n","\n","Given that:\n","* $\\lim_{h\\to0}e^h-1=\\lim_{y\\to0}y$\n","\n","$\\therefore \\lim_{h\\to0}\\frac{e^{h}-1}{h}=\\lim_{y\\to0}\\frac{y}{\\log_e(y+1)}$\n","\n","$\\lim_{y\\to0}\\frac{y}{\\ln(y+1)}=\\lim_{y\\to0}\\frac{1}{\\frac{\\ln(y+1)}{y}}$\n","\n","$\\lim_{y\\to0}\\frac{y}{\\ln(y+1)}=\\lim_{y\\to0}\\frac{1}{\\frac{1}{y}*\\ln(y+1)}$\n","\n","\n","According to Logarithm property: $\\log_a(x^y)=y*\\log_a(x)=\\log_a(x)*y$\n","\n","$\\therefore\\lim_{y\\to0}\\frac{y}{\\ln(y+1)}=\\lim_{y\\to0}\\frac{1}{\\ln((y+1)^\\frac{1}{y})}$\n","\n","Given that\n","* $\\lim_{n\\to\\infty}(1+\\frac{1}{n})^n=e$\n","* $\\lim_{n\\to\\infty}\\frac{1}{n}=\\lim_{y\\to0}y$\n","* $\\therefore \\lim_{n\\to\\infty}(1+\\frac{1}{n})^n=\\lim_{y\\to0}(y+1)^\\frac{1}{y}=e$\n","\n","$\\therefore\\lim_{y\\to0}\\frac{y}{\\ln(y+1)}=\\frac{1}{\\ln(e)}$\n","\n","According to Logarithm property: $\\log_aa^x=x$\n","\n","$\\therefore\\lim_{y\\to0}\\frac{y}{\\ln(y+1)}=\\frac{1}{1}=1$\n","\n","reference:\n","* https://youtu.be/qWw8VnzTddg\n","* https://socratic.org/questions/how-do-you-solve-the-following-limit-e-x-1-x-as-x-approaches-zero"],"metadata":{"id":"7rJUQgU0Xohu"}},{"cell_type":"markdown","source":["**Proof No.2: $\\lim_{h\\to0}\\frac{c^{h}-1}{h}=\\log_e(c)=\\ln(c)$**\n","\n","Given that:\n","* $y=c^h-1$\n","\n","$y+1=c^h$\n","\n","$\\ln(y+1)=\\ln(c^h)$\n","\n","According to Logarithm: $\\log_a(x^y)=y*\\log_a(x)=\\log_a(x)*y$\n","\n","$\\therefore\\ln(y+1)=h*\\ln(c)$\n","\n","$\\frac{\\ln(y+1)}{\\ln(c)}=h$\n","\n","Given that:\n","* $y=c^h-1$\n","* $\\frac{\\ln(y+1)}{\\ln(c)}=h$\n","\n","$\\therefore \\frac{c^h-1}{h}=\\frac{y}{\\frac{\\ln(y+1)}{\\ln(c)}}$\n","\n","$\\frac{c^h-1}{h}=\\frac{y}{\\ln(y+1)}*\\ln(c)$\n","\n","\n","reference:\n","* https://math.stackexchange.com/questions/331153/proving-that-lim-h-to-0-fracbh-1h-lnb"],"metadata":{"id":"N6JQ6fyedivN"}},{"cell_type":"markdown","source":["**Prove that $\\lim_{h \\to 0}\\frac{e^{h}-1}{h}=1$ No.1**"],"metadata":{"id":"vc3gUk7UdmMj"}},{"cell_type":"markdown","source":["###To Do Now\n","* Fractional Binomial Theorem, Alternative Binomial Theorem Proof\n","* Integral\n","* $\\frac{d}{dx}[f(x)^{g(x)}]$, Proof that: $\\lim_{h\\to0}\\frac{x^{h}-1}{h}=\\ln(x)$\n","* d7.ipynb: $f(f(x))+f(x)=1,\\{x\\in\\mathbb{R},f(x)=?\\}$"],"metadata":{"id":"PrlepTH5E-Y9"}}]}