{"nbformat":4,"nbformat_minor":0,"metadata":{"colab":{"provenance":[],"authorship_tag":"ABX9TyOkqcCrxz402IjJc2x5Noeb"},"kernelspec":{"name":"python3","display_name":"Python 3"},"language_info":{"name":"python"}},"cells":[{"cell_type":"markdown","source":["###(1): $f(f(x))+x*f(x)=1,x\\in\\mathbb{R},f(x)=?$"],"metadata":{"id":"nkRSwdGYa4t_"}},{"cell_type":"markdown","source":["$f(x)=mx+\\frac{1-mx(x+m)}{m+x+1}$\n","\n","$f(f(x))=m*f(x)+\\frac{1-m*f(x)*(f(x)+m)}{m+f(x)+1}$\n","\n","$f(f(x))+x*f(x)-1\n","=m*f(x)+\\frac{1-m*f(x)*(f(x)+m)}{m+f(x)+1}\n","+mx^2+\\frac{x-mx^2(x+m)}{m+x+1}\n","-1$\n","\n","$f(f(x))+x*f(x)-1\n","=m^2x+\\frac{m-m^2x(x+m)}{m+x+1}\n","+\\frac{1-m*f(x)*(f(x)+m)}{m+f(x)+1}\n","+mx^2+\\frac{x-mx^2(x+m)}{m+x+1}\n","-1$\n","\n","$f(f(x))+x*f(x)-1\n","=m^2x+\\frac{m-m^2x(x+m)}{m+x+1}\n","+mx^2+\\frac{x-mx^2(x+m)}{m+x+1}\n","-1+\\frac{1-m*f(x)*(f(x)+m)}{m+f(x)+1}$\n","\n","$f(f(x))+x*f(x)-1\n","=m^2x+mx^2\n","+\\frac{m-m^2x(x+m)+x-mx^2(x+m)}{m+x+1}\n","+\\frac{1-m*f(x)*(f(x)+m)}{m+f(x)+1}-1$\n","\n","$f(f(x))+x*f(x)-1\n","=m^2x+mx^2\n","+\\frac{m-m^2x^2-m^3x+x-mx^3-m^2x^2}{m+x+1}\n","+\\frac{1-m*f(x)*(f(x)+m)}{m+f(x)+1}-1$\n","\n","$f(f(x))+x*f(x)-1\n","=m^2x+mx^2\n","+\\frac{m+x-m^3x-mx^3-2m^2x^2}{m+x+1}\n","+\\frac{1-m*f(x)*(f(x)+m)}{m+f(x)+1}-1$"],"metadata":{"id":"4msCWRrqmeEF"}},{"cell_type":"markdown","source":["**Note:**\n","\n","Lagrange's notation of multiple order derivative\n","* $f^{(1)}(x)=f'(x)$\n","* $f^{(2)}(x)=f''(x)$\n","* $f^{(n)}(x)=f''^{...}(x)$\n","\n","My notation of nested function\n","* $f^{[1]}(x)=f(x)$\n","* $f^{[2]}(x)=f(f(x))$\n","* $f^{[n]}(x)=f(f(f(...f(x)...)))$\n","\n","reference:\n","* https://en.wikipedia.org/wiki/Notation_for_differentiation"],"metadata":{"id":"CWu3BUel_He8"}},{"cell_type":"markdown","source":["**Solution No.1**\n","\n","Given that: $f(f(x))+x*f(x)=f^{[2]}(x)+x*f(x)=1$\n","\n","If: $x=0$\n","* $f^{[2]}(0)+0*f(0)=1$\n","* $\\therefore f(f(0))=f^{[2]}(0)=1$\n","\n","If: $x=f(0)$\n","* $f^{[2]}(f(0))+f(0)*f(f(0))=1$\n","* $f^{[3]}(0)+f(0)*f^{[2]}(0)=1$\n","* Given that: $f^{[2]}(0)=1$\n","* $\\therefore f^{[3]}(0)+f(0)=1$\n","* $f^{[1]}(f^{[2]}(0))+f(0)=1$\n","* $f^{[1]}(1)+f(0)=1$\n","* $f(1)+f(0)=1$\n","\n","If: $x=1$\n","* $f^{[2]}(1)+1*f(1)=1$\n","* $f^{[2]}(1)+f(1)=1$\n","* Given that: $f(1)+f(0)=f^{[2]}(1)+f(1)=1$\n","* $\\therefore f(0)=f^{[2]}(1)=1-f(1)$\n","\n","If: $x=f(1)$\n","* $f^{[2]}(f(1))+f(1)*f(f(1))=1$\n","* $f^{[3]}(1)+f(1)*f^{[2]}(1)=1$\n","* Given that: $f(0)=f^{[2]}(1)$\n","* $\\therefore f^{[3]}(1)+f(1)*f(0)=1$\n","* $f^{[1]}(f^{[2]}(1))+f(1)*f(0)=1$\n","* $f^{[1]}(f(0))+f(1)*f(0)=1$\n","* $f^{[2]}(0)+f(1)*f(0)=1$\n","* Given that: $f^{[2]}(0)=1$\n","* $\\therefore 1+f(1)*f(0)=1$\n","* $f(1)*f(0)=0$\n","* $\\therefore f(0)=0\\lor f(1)=0$\n","\n","If $f(0)=0$\n","* Given that: $f(1)+f(0)=1\\implies f(1)=1$\n","* Given that: $f(0)=f^{[2]}(1)\\implies f^{[2]}(1)=0$\n","* Given that: $f^{[2]}(1)=0\\land f(1)=1\\implies f(f(x))=f(1)=0$\n","* $\\therefore f(0)\\neq0$\n","\n","If $f(1)=0$\n","* Given that: $f(1)+f(0)=1\\implies f(0)=1$\n","* Given that: $f^{[2]}(0)=1\\implies f(f(0))=f(1)=1$\n","* $\\therefore f(1)\\neq0$\n","* $\\therefore f=\\{\\}$\n","\n","**Answer: No Answer**"],"metadata":{"id":"rv5cCJxPCUh-"}},{"cell_type":"markdown","source":["$(x^2+1)-x^2=1$\n","\n","$\\frac{a}{y}+\\frac{xb}{y}=1\\implies a+xb=y$\n"],"metadata":{"id":"wzSvMTXrgaoH"}},{"cell_type":"markdown","source":["**Unfinished: Do This First**\n","\n","**Solution No.2**\n","\n","Given that:\n","* $f^{[2]}(x)+x*f(x)=1$\n","* $f(x)=\\frac{g(x)}{r}$\n","* $\\therefore f^{[2]}(x)+x*f(x)=\\frac{g(f(x))+x*g(x)}{r}=1$\n","* $\\therefore g(f(x))+x*g(x)=r$\n","* $r=g(\\frac{g(x)}{r})+x*g(x)=g(\\frac{g(x)}{g(\\frac{g(x)}{g(...)+x*g(x)})+x*g(x)})+x*g(x)$\n","\n","If: $x=0$\n","* $\\frac{g(f(0))+0*g(0)}{r}=1$\n","* $\\frac{g(f(0))}{r}=1\\implies r=g(f(0))$\n","\n","If: $x=f(0)$\n","* $\\frac{g(f(f(0)))+f(0)*g(f(0))}{r}=1$\n","* $\\frac{g(f^{[2]}(0))+f(0)*g(f(0))}{r}=1$\n","* $r=g(f^{[2]}(0))+f(0)*g(f(0))$\n","* Given that: $r=g(f(0))\\implies r=g(f^{[2]}(0))+f(0)*r$\n","* $0=g(f^{[2]}(0))+f(0)*r-r$\n","* $0=g(f^{[2]}(0))+(f(0)-1)*r$\n","* $-(f(0)-1)*r=g(f^{[2]}(0))$\n","* $(f(0)-1)*r=-g(f^{[2]}(0))$\n","* $r=\\frac{-g(f^{[2]}(0))}{f(0)-1}$\n","\n","If: $x=g(0)$\n","* $g(f(g(0)))+x*g(g(0))=r$\n","* $g(f(g(0)))+x*g^{[2]}(0))=r$\n","* ...\n","\n","If: $x=1$\n","* $\\frac{g(f(1))+g(1)}{r}=1$\n","* $\\therefore r=g(f(1))+g(1)$\n","\n","If: $x=f(1)$\n","* $g(f(f(1)))+x*g(f(1))=r$\n","* $g(f^{[2]}(1))+x*g(f(1))=r$\n","* Given that: $r=g(f(0))\\implies $\n","\n","If: $x=2$\n","* $\\frac{g(f(2))+2*g(2)}{r}=1$\n","* $\\therefore r=g(f(2))+2*g(2)$"],"metadata":{"id":"cfMGpxEzhQJD"}},{"cell_type":"markdown","source":["**Unfinished**\n","\n","**Solution No.2**\n","\n","Given that:\n","* $f^{[2]}(x)+x*f(x)=1$\n","* $f(x)=\\frac{g(x)}{r}$\n","* $\\therefore f^{[2]}(x)+x*f(x)=\\frac{g(f(x))+x*g(x)}{r}=1$\n","* $\\therefore r=g(f(x))+x*g(x)$\n","* $r=g(\\frac{g(x)}{r})+x*g(x)=g(\\frac{g(x)}{g(\\frac{g(x)}{g(...)+x*g(x)})+x*g(x)})+x*g(x)$\n","\n","If: $x=0$\n","* $\\frac{g(f(0))+0*g(0)}{r}=1$\n","* $\\frac{g(f(0))}{r}=1\\implies r=g(f(0))$\n","\n","If: $x=1$\n","* $\\frac{g(f(1))+g(1)}{r}=1$\n","* $\\therefore r=g(f(1))+g(1)$\n","\n","If: $x=2$\n","* $\\frac{g(f(2))+2*g(2)}{r}=1$\n","* $\\therefore r=g(f(2))+2*g(2)$"],"metadata":{"id":"0Zl3_e-OX74x"}},{"cell_type":"markdown","source":["**Unfinished**\n","\n","**Solution No.2**\n","\n","Given that:\n","* $f^{[m+1]}(x)+x*f^{[m]}(x)=1$\n","* $m\\in\\mathbb{Z}$\n","* $x,f(x)\\in\\mathbb{R}$\n","\n","$\\therefore f^{[2m]}(x)+x*f^{2m-1}(x)=1$\n","\n","$f(x)=-1*(g(x))$"],"metadata":{"id":"lVl5LVFzUrZn"}},{"cell_type":"markdown","source":["**Unfinished**\n","\n","**Solution No.2**\n","\n","Given that:\n","* $f^{[2]}(x)+x*f(x)=1$\n","* $m\\in\\mathbb{Z}$\n","* $x,f(x)\\in\\mathbb{R}$\n","* $f^{[2m-1]}(x)\\leq0$\n","* $f^{[2m]}(x)\\geq0$\n","\n","$\\therefore f^{[2m]}(x)+x*f^{2m-1}(x)=1$\n","\n","$f(x)=-1*(g(x))$"],"metadata":{"id":"xi-fj_smb36T"}},{"cell_type":"markdown","source":["reference: https://youtu.be/jb1J7Dcmu3Y"],"metadata":{"id":"UWl6aVwEbPR-"}},{"cell_type":"markdown","source":["###(1.1): $f(f(x))+f(x)=1,\\{x\\in\\mathbb{R},f(x)=?\\}$"],"metadata":{"id":"g_-7EF88T0Cc"}},{"cell_type":"markdown","source":["###(1.2): $f(f(x))+f(x)=y,x\\in\\mathbb{R},f(x)=?$\n"],"metadata":{"id":"_2Ipjy3rT6de"}},{"cell_type":"markdown","source":["###(2): $f(x)+f(\\frac{1}{1-x})=x$"],"metadata":{"id":"2RbrDY75nE0c"}},{"cell_type":"markdown","source":["reference: https://youtu.be/oNT4iwU6Pew"],"metadata":{"id":"oLJQbqNGokkr"}},{"cell_type":"markdown","source":["###A: $f^{(n),[m]}(x)=?$"],"metadata":{"id":"m640jzT-E61K"}},{"cell_type":"markdown","source":["###B: $f^{(\\frac{n}{m})}(x)=?$"],"metadata":{"id":"BfseWPVCHuih"}},{"cell_type":"markdown","source":["###C: $f^{[\\frac{n}{m}]}(x)=?$\n"],"metadata":{"id":"ilmAeZg6H3HZ"}}]}